NuSys.thy
@@ -44,7 +44,239 @@ declare [ [ML_debugger, ML_exception_debugger] ]
 
 chapter \<open>An Interactive Programming Language embedded in Isar\<close>
 
-section \<open>Basic Structures & Features of Deductive Programming\<close>
+section \<open>\<phi>-Type\<close>
+
+type_synonym ('concrete,'abstract) \<phi> = " 'abstract \<Rightarrow> 'concrete set "
+
+
+subsubsection \<open>Definitions\<close>
+
+definition \<phi>Type :: "'b \<Rightarrow> ('a,'b) \<phi> \<Rightarrow> 'a set" (infix "\<Ztypecolon>" 20) where " (x \<Ztypecolon> T) = (T x)"
+
+lemma typing_inhabited: "p \<in> (x \<Ztypecolon> T) \<Longrightarrow> Inhabited (x \<Ztypecolon> T)"
+  unfolding Inhabited_def \<phi>Type_def by blast
+
+lemma \<phi>Type_eqI:
+  \<open>(\<forall>x p. p \<in> (x \<Ztypecolon> a) \<longleftrightarrow> p \<in> (x \<Ztypecolon> b)) \<Longrightarrow> a = b\<close>
+  unfolding \<phi>Type_def by blast
+
+
+
+paragraph \<open>Syntax\<close>
+
+abbreviation (in std) COMMA
+  :: \<open>('FIC_N,'FIC) assn \<Rightarrow> ('FIC_N,'FIC) assn \<Rightarrow> ('FIC_N,'FIC) assn\<close> (infixl "\<heavy_comma>" 13)
+  where \<open>COMMA \<equiv> (*)\<close>
+
+(*
+setup \<open>(Sign.add_trrules (let open Ast 
+      fun nuty x y = Appl [Constant \<^const_syntax>\<open>\<phi>Type\<close>, Variable x, Variable y]
+      fun wrap_ele tm = Appl [Constant \<^const_syntax>\<open>Ele\<close>, tm]
+      fun wrap_nuty x y = wrap_ele (nuty x y)
+    in [
+      Syntax.Parse_Print_Rule (
+        Appl [Constant "\<^const>local.COMMA", nuty "x" "T", Variable "U"],
+        Appl [Constant "\<^const>local.COMMA", wrap_nuty "x" "T", Variable "U"]),
+      Syntax.Parse_Print_Rule (
+        Appl [Constant "\<^const>local.COMMA", Variable "U", nuty "x" "T"],
+        Appl [Constant "\<^const>local.COMMA", Variable "U", wrap_nuty "x" "T"]),
+      Syntax.Parse_Print_Rule (
+        Appl [Constant "\<^const>local.\<phi>Procedure", Variable "f", nuty "x" "T", Variable "U"],
+        Appl [Constant "\<^const>local.\<phi>Procedure", Variable "f", wrap_nuty "x" "T", Variable "U"]),
+      Syntax.Parse_Print_Rule (
+        Appl [Constant "\<^const>local.\<phi>Procedure", Variable "f", Variable "U", nuty "x" "T"],
+        Appl [Constant "\<^const>local.\<phi>Procedure", Variable "f", Variable "U", wrap_nuty "x" "T"]),
+      Syntax.Parse_Print_Rule (
+        Appl [Constant "\<^const>local.\<phi>Procedure_no_exception", Variable "f", nuty "x" "T", Variable "U"],
+        Appl [Constant "\<^const>local.\<phi>Procedure_no_exception", Variable "f", wrap_nuty "x" "T", Variable "U"]),
+      Syntax.Parse_Print_Rule (
+        Appl [Constant "\<^const>local.\<phi>Procedure_no_exception", Variable "f", Variable "U", nuty "x" "T"],
+        Appl [Constant "\<^const>local.\<phi>Procedure_no_exception", Variable "f", Variable "U", wrap_nuty "x" "T"]),
+      Syntax.Parse_Print_Rule (
+        Appl [Constant "\<^const>local.CurrentConstruction", Variable "s", Variable "R", nuty "x" "T"],
+        Appl [Constant "\<^const>local.CurrentConstruction", Variable "s", Variable "R", wrap_nuty "x" "T"]),
+      Syntax.Parse_Print_Rule (
+        Appl [Constant "\<^const>local.PendingConstruction", Variable "f", Variable "s", Variable "R", nuty "x" "T"],
+        Appl [Constant "\<^const>local.PendingConstruction", Variable "f", Variable "s", Variable "R", wrap_nuty "x" "T"])
+  ] end))\<close>
+*)
+
+subsubsection \<open>Properties\<close>
+
+context std_sem begin
+
+definition \<phi>SemType :: "'VAL set \<Rightarrow> 'TY \<Rightarrow> bool"
+  where [\<phi>def]: \<open>\<phi>SemType S TY \<longleftrightarrow> S \<subseteq> Well_Type TY\<close>
+
+abbreviation \<phi>\<phi>SemType :: "('VAL, 'a) \<phi> \<Rightarrow> 'TY \<Rightarrow> bool"
+  where \<open>\<phi>\<phi>SemType T TY \<equiv> (\<forall>x. \<phi>SemType (x \<Ztypecolon> T) TY)\<close>
+
+definition \<phi>Zero :: "'TY \<Rightarrow> ('VAL,'a) \<phi> \<Rightarrow> 'a \<Rightarrow> bool"
+  where [\<phi>def]: "\<phi>Zero ty T x \<longleftrightarrow> Zero ty \<in> (x \<Ztypecolon> T)"
+
+definition \<phi>Equal :: "('VAL,'a) \<phi> \<Rightarrow> ('a \<Rightarrow> 'a \<Rightarrow> bool) \<Rightarrow> ('a \<Rightarrow> 'a \<Rightarrow> bool) \<Rightarrow> bool"
+  where [\<phi>def]: "\<phi>Equal T can_eq eq \<longleftrightarrow> (\<forall>p1 p2 x1 x2 res.
+    can_eq x1 x2 \<and> p1 \<in> (x1 \<Ztypecolon> T) \<and> p2 \<in> (x2 \<Ztypecolon> T)
+      \<longrightarrow> Can_EqCompare res p1 p2 \<and> (EqCompare p1 p2 = eq x1 x2))"
+
+end
+
+definition Subty :: " 'a set \<Rightarrow> 'a set \<Rightarrow> bool \<Rightarrow> bool " ("(2\<^bold>s\<^bold>u\<^bold>b\<^bold>t\<^bold>y\<^bold>p\<^bold>e _/ \<longmapsto> _/ \<^bold>w\<^bold>i\<^bold>t\<^bold>h _)" [13,13,13] 12)
+  where "(\<^bold>s\<^bold>u\<^bold>b\<^bold>t\<^bold>y\<^bold>p\<^bold>e A \<longmapsto> B \<^bold>w\<^bold>i\<^bold>t\<^bold>h P) \<longleftrightarrow> (\<forall>v. v \<in> A \<longrightarrow> v \<in> B \<and> P)"
+
+consts SimpleSubty :: " 'a set \<Rightarrow> 'a set \<Rightarrow> bool \<Rightarrow> bool " ("(2\<^bold>s\<^bold>u\<^bold>b\<^bold>t\<^bold>y\<^bold>p\<^bold>e _/ \<longmapsto> _)" [13,13] 12)
+translations "(\<^bold>s\<^bold>u\<^bold>b\<^bold>t\<^bold>y\<^bold>p\<^bold>e A \<longmapsto> B)" == "(\<^bold>s\<^bold>u\<^bold>b\<^bold>t\<^bold>y\<^bold>p\<^bold>e A \<longmapsto> B \<^bold>w\<^bold>i\<^bold>t\<^bold>h CONST True)"
+
+
+subsubsection \<open>Subjection\<close>
+
+definition Subjection :: " 'p set \<Rightarrow> bool \<Rightarrow> 'p set " (infixl "\<^bold>s\<^bold>u\<^bold>b\<^bold>j" 13)
+  where " (T \<^bold>s\<^bold>u\<^bold>b\<^bold>j P) = {p. p \<in> T \<and> P}"
+
+lemma Subjection_expn[\<phi>expns]:
+  "p \<in> (T \<^bold>s\<^bold>u\<^bold>b\<^bold>j P) \<longleftrightarrow> p \<in> T \<and> P"
+  unfolding Subjection_def by simp
+
+lemma Subjection_inhabited[elim!,\<phi>reason_elim!]:
+  \<open>Inhabited (S \<^bold>s\<^bold>u\<^bold>b\<^bold>j P) \<Longrightarrow> (P \<Longrightarrow> Inhabited S \<Longrightarrow> C) \<Longrightarrow> C\<close>
+  unfolding Inhabited_def by (simp add: \<phi>expns)
+
+lemma [\<phi>reason]:
+  " \<^bold>s\<^bold>u\<^bold>b\<^bold>t\<^bold>y\<^bold>p\<^bold>e T \<longmapsto> T' \<^bold>w\<^bold>i\<^bold>t\<^bold>h P
+\<Longrightarrow> (P \<Longrightarrow> \<^bold>p\<^bold>r\<^bold>e\<^bold>m\<^bold>i\<^bold>s\<^bold>e Q)
+\<Longrightarrow> \<^bold>s\<^bold>u\<^bold>b\<^bold>t\<^bold>y\<^bold>p\<^bold>e T \<longmapsto> T' \<^bold>s\<^bold>u\<^bold>b\<^bold>j Q \<^bold>w\<^bold>i\<^bold>t\<^bold>h P"
+  unfolding Subty_def Premise_def by (simp add: \<phi>expns)
+
+lemma [simp]: "(T \<^bold>s\<^bold>u\<^bold>b\<^bold>j True) = T" by (auto simp add: \<phi>expns)
+(* lemma (in std) [simp]: "(VAL (S \<^bold>s\<^bold>u\<^bold>b\<^bold>j P)) = (VAL S \<^bold>s\<^bold>u\<^bold>b\<^bold>j P)" by (simp add: \<phi>expns set_eq_iff) blast
+lemma (in std) [simp]: "(OBJ (S \<^bold>s\<^bold>u\<^bold>b\<^bold>j P)) = (OBJ S \<^bold>s\<^bold>u\<^bold>b\<^bold>j P)" by (simp add: \<phi>expns set_eq_iff) *)
+
+lemma Subjection_times[simp]:
+  \<open>(S \<^bold>s\<^bold>u\<^bold>b\<^bold>j P) * T = (S * T \<^bold>s\<^bold>u\<^bold>b\<^bold>j P)\<close>
+  \<open>T * (S \<^bold>s\<^bold>u\<^bold>b\<^bold>j P) = (T * S \<^bold>s\<^bold>u\<^bold>b\<^bold>j P)\<close>
+  unfolding Subjection_def times_set_def set_eq_iff by blast+
+
+
+(* declare split_paired_All[simp del] split_paired_Ex[simp del] *)
+
+lemma (in std) Subjection_simp_proc_arg'[simp]:
+  "\<^bold>p\<^bold>r\<^bold>o\<^bold>c f \<lbrace> T \<^bold>s\<^bold>u\<^bold>b\<^bold>j P \<longmapsto> Y \<^bold>t\<^bold>h\<^bold>r\<^bold>o\<^bold>w\<^bold>s E \<rbrace> = (P \<longrightarrow> \<^bold>p\<^bold>r\<^bold>o\<^bold>c f \<lbrace> T \<longmapsto> Y \<^bold>t\<^bold>h\<^bold>r\<^bold>o\<^bold>w\<^bold>s E \<rbrace>)"
+  (* and Subjection_simp_func_arg[simp]: "\<^bold>f\<^bold>u\<^bold>n\<^bold>c f' \<lbrace> T \<and>\<^sup>s P \<longmapsto> Y \<rbrace> = (P \<longrightarrow> \<^bold>f\<^bold>u\<^bold>n\<^bold>c f' \<lbrace> T \<longmapsto> Y \<rbrace>)" *)
+  unfolding \<phi>Procedure_def by (simp add: \<phi>expns) blast
+
+lemmas (in std) Subjection_simp_proc_arg[unfolded atomize_eq[symmetric]] = Subjection_simp_proc_arg'
+
+
+(* ML \<open>Theory.setup (Sign.add_trrules (let open Ast 
+      fun nuty x y = Appl [Constant \<^const_syntax>\<open>\<phi>Type\<close>, Variable x, Variable y]
+      fun wrap_ele tm = Appl [Constant \<^const_syntax>\<open>Ele\<close>, tm]
+      fun wrap_nuty x y = wrap_ele (nuty x y)
+      fun subj x = Appl [Constant \<^const_syntax>\<open>Subjection\<close>, x, Variable "P"]
+    in [
+      Syntax.Parse_Print_Rule (
+        Appl [Constant "\<^const>local.\<phi>Procedure", Variable "f", subj (nuty "x" "T"), Variable "U"],
+        Appl [Constant "\<^const>local.\<phi>Procedure", Variable "f", subj (wrap_nuty "x" "T"), Variable "U"]),
+      Syntax.Parse_Print_Rule (
+        Appl [Constant "\<^const>local.\<phi>Procedure", Variable "f", Variable "U", subj (nuty "x" "T")],
+        Appl [Constant "\<^const>local.\<phi>Procedure", Variable "f", Variable "U", subj (wrap_nuty "x" "T")]),
+      Syntax.Parse_Print_Rule (
+        Appl [Constant "\<^const>local.\<phi>Procedure_no_exception", Variable "f", subj (nuty "x" "T"), Variable "U"],
+        Appl [Constant "\<^const>local.\<phi>Procedure_no_exception", Variable "f", subj (wrap_nuty "x" "T"), Variable "U"]),
+      Syntax.Parse_Print_Rule (
+        Appl [Constant "\<^const>local.\<phi>Procedure_no_exception", Variable "f", Variable "U", subj (nuty "x" "T")],
+        Appl [Constant "\<^const>local.\<phi>Procedure_no_exception", Variable "f", Variable "U", subj (wrap_nuty "x" "T")])
+  ] end))\<close>
+*)
+
+
+subsubsection \<open>Existential Quantification\<close>
+
+definition ExSet :: " ('c \<Rightarrow> 'a set) \<Rightarrow> 'a set" (binder "\<exists>*" 10)
+  where "ExSet S = {p. (\<exists>c. p \<in> S c)}"
+notation ExSet (binder "\<exists>\<^sup>s" 10)
+
+
+lemma [\<phi>expns]: "p \<in> ExSet S \<longleftrightarrow> (\<exists>c. p \<in> S c)" unfolding ExSet_def by simp
+
+syntax
+  "_SetcomprNu" :: "'a \<Rightarrow> idts \<Rightarrow> bool \<Rightarrow> 'a set"  ("_ \<^bold>s\<^bold>u\<^bold>b\<^bold>j/ _./ _" [3,0,4] 3)
+
+translations
+  " X \<^bold>s\<^bold>u\<^bold>b\<^bold>j idts. P " \<rightleftharpoons> "\<exists>* idts. X \<^bold>s\<^bold>u\<^bold>b\<^bold>j P"
+  " X \<^bold>s\<^bold>u\<^bold>b\<^bold>j idts. CONST True " \<rightleftharpoons> "\<exists>* idts. X"
+
+
+(*
+ML \<open>Theory.setup (Sign.add_trrules (let open Ast 
+      fun nuty x y = Appl [Constant \<^const_syntax>\<open>\<phi>Type\<close>, Variable x, Variable y]
+      fun wrap_ele tm = Appl [Constant \<^const_syntax>\<open>Ele\<close>, tm]
+      fun wrap_nuty x y = wrap_ele (nuty x y)
+      fun subj x = Appl [Constant \<^syntax_const>\<open>_SetcomprNu\<close>, x, Variable "idts", Variable "P"]
+    in [
+      Syntax.Parse_Print_Rule (
+        Appl [Constant "\<^const>local.\<phi>Procedure", Variable "f", subj (nuty "x" "T"), Variable "U"],
+        Appl [Constant "\<^const>local.\<phi>Procedure", Variable "f", subj (wrap_nuty "x" "T"), Variable "U"]),
+      Syntax.Parse_Print_Rule (
+        Appl [Constant "\<^const>local.\<phi>Procedure", Variable "f", Variable "U", subj (nuty "x" "T")],
+        Appl [Constant "\<^const>local.\<phi>Procedure", Variable "f", Variable "U", subj (wrap_nuty "x" "T")]),
+      Syntax.Parse_Print_Rule (
+        Appl [Constant "\<^const>local.\<phi>Procedure_no_exception", Variable "f", subj (nuty "x" "T"), Variable "U"],
+        Appl [Constant "\<^const>local.\<phi>Procedure_no_exception", Variable "f", subj (wrap_nuty "x" "T"), Variable "U"]),
+      Syntax.Parse_Print_Rule (
+        Appl [Constant "\<^const>local.\<phi>Procedure_no_exception", Variable "f", Variable "U", subj (nuty "x" "T")],
+        Appl [Constant "\<^const>local.\<phi>Procedure_no_exception", Variable "f", Variable "U", subj (wrap_nuty "x" "T")])
+  ] end))\<close>
+*)
+text (in std)
+ \<open>The set of \<phi>-type in an assertion like \<^term>\<open>\<^bold>p\<^bold>r\<^bold>o\<^bold>c f \<lbrace> S x \<^bold>s\<^bold>u\<^bold>b\<^bold>j x. P x \<longmapsto> \<lambda>ret. T x \<^bold>s\<^bold>u\<^bold>b\<^bold>j x. Q x \<rbrace>\<close> is represented
+  by \<^const>\<open>ExSet\<close> and we show a \<phi>-type \<^term>\<open>S x \<^bold>s\<^bold>u\<^bold>b\<^bold>j x. P x\<close> represents actually all concrete values that
+  belongs to \<^term>\<open>S\<close> a set of \<phi>-types (i.e. the union of \<^term>\<open>S\<close>) by following lemma\<close>
+
+lemma " Union { S x |x. P x } = (S x \<^bold>s\<^bold>u\<^bold>b\<^bold>j x. P x) "
+  by (simp add: set_eq_iff \<phi>expns) blast
+
+
+lemma ExSet_pair: "ExSet T = (\<exists>*c1 c2. T (c1,c2) )" by (auto simp add: \<phi>expns)
+
+(* lemma (in std_sem) [simp]: "p \<in> \<S>  (ExSet T) \<longleftrightarrow> (\<exists>z. p \<in> \<S>  (T z) )" by (cases p, simp_all add: \<phi>expns set_eq_iff)
+lemma (in std_sem) [simp]: "p \<in> !\<S> (ExSet T) \<longleftrightarrow> (\<exists>z. p \<in> !\<S> (T z) )" by (cases p, simp_all add: \<phi>expns set_eq_iff) *)
+(* lemma (in std) [simp]: "(VAL ExSet T) = (\<exists>*c. VAL T c)" by (simp add: \<phi>expns set_eq_iff) blast
+lemma (in std) [simp]: "(OBJ ExSet T) = (\<exists>*c. OBJ T c)" by (simp add: \<phi>expns set_eq_iff) *)
+lemma [simp]: "(ExSet T * R) = (\<exists>* c. T c * R )" by (simp add: \<phi>expns set_eq_iff) blast
+lemma ExSet_times[simp]: "(L * ExSet T) = (\<exists>* c. L * T c)" by (simp add: \<phi>expns set_eq_iff) blast
+
+lemma ExSet_ExSet[simp]:
+  \<open>(X a b \<^bold>s\<^bold>u\<^bold>b\<^bold>j a. P a b \<^bold>s\<^bold>u\<^bold>b\<^bold>j b. Q b) = (X a b \<^bold>s\<^bold>u\<^bold>b\<^bold>j a b. P a b \<and> Q b)\<close>
+  unfolding set_eq_iff by (simp add: \<phi>expns, blast)
+
+lemma ExSet_SubjSet[simp]:
+  \<open>(X b \<^bold>s\<^bold>u\<^bold>b\<^bold>j P b \<^bold>s\<^bold>u\<^bold>b\<^bold>j b. Q b) = (X b \<^bold>s\<^bold>u\<^bold>b\<^bold>j b. P b \<and> Q b)\<close>
+  unfolding set_eq_iff by (simp add: \<phi>expns)
+
+lemma [\<phi>reason 200]: "(\<And>c. \<^bold>s\<^bold>u\<^bold>b\<^bold>t\<^bold>y\<^bold>p\<^bold>e T c \<longmapsto> T' \<^bold>w\<^bold>i\<^bold>t\<^bold>h P c) \<Longrightarrow> \<^bold>s\<^bold>u\<^bold>b\<^bold>t\<^bold>y\<^bold>p\<^bold>e (ExSet T) \<longmapsto> T' \<^bold>w\<^bold>i\<^bold>t\<^bold>h (\<exists>c. P c)"
+  unfolding Subty_def by (simp add: \<phi>expns) blast
+
+subsubsection \<open>Simplification & Reasoning\<close>
+
+lemma (in std) \<phi>CONSEQ':
+   "\<^bold>s\<^bold>u\<^bold>b\<^bold>t\<^bold>y\<^bold>p\<^bold>e A' \<longmapsto> A \<^bold>w\<^bold>i\<^bold>t\<^bold>h P1
+\<Longrightarrow> (\<And>x. \<^bold>s\<^bold>u\<^bold>b\<^bold>t\<^bold>y\<^bold>p\<^bold>e B x \<longmapsto> B' x \<^bold>w\<^bold>i\<^bold>t\<^bold>h P2)
+\<Longrightarrow> \<^bold>s\<^bold>u\<^bold>b\<^bold>t\<^bold>y\<^bold>p\<^bold>e E \<longmapsto> E' \<^bold>w\<^bold>i\<^bold>t\<^bold>h P3
+\<Longrightarrow> \<^bold>p\<^bold>r\<^bold>o\<^bold>c f \<lbrace> A  \<longmapsto> B  \<^bold>t\<^bold>h\<^bold>r\<^bold>o\<^bold>w\<^bold>s E  \<rbrace>
+\<Longrightarrow> \<^bold>p\<^bold>r\<^bold>o\<^bold>c f \<lbrace> A' \<longmapsto> B' \<^bold>t\<^bold>h\<^bold>r\<^bold>o\<^bold>w\<^bold>s E' \<rbrace>"
+  unfolding Subty_def
+  by (meson \<phi>CONSEQ subsetI)
+
+lemma (in std) \<phi>CONSEQ'E:
+   "\<^bold>s\<^bold>u\<^bold>b\<^bold>t\<^bold>y\<^bold>p\<^bold>e E \<longmapsto> E' \<^bold>w\<^bold>i\<^bold>t\<^bold>h P3
+\<Longrightarrow> \<^bold>p\<^bold>r\<^bold>o\<^bold>c f \<lbrace> A  \<longmapsto> B  \<^bold>t\<^bold>h\<^bold>r\<^bold>o\<^bold>w\<^bold>s E  \<rbrace>
+\<Longrightarrow> \<^bold>p\<^bold>r\<^bold>o\<^bold>c f \<lbrace> A \<longmapsto> B \<^bold>t\<^bold>h\<^bold>r\<^bold>o\<^bold>w\<^bold>s E' \<rbrace>"
+  unfolding Subty_def
+  by (meson \<phi>CONSEQ subsetI)
+
+
+
+section \<open>Basic Constructions of the Deductive Programming\<close>
 
 
 subsection \<open>Preliminary\<close>
@@ -58,9 +290,14 @@ and \<phi>lemmata \<open>Contextual facts during the programming. They are autom
        cleared frequently\<close> 
 
 ML_file NuHelp.ML
+ML_file \<open>library/NuSimpCongruence.ML\<close>
 
+subsubsection \<open>Reasoning Tags\<close>
 
-subsection \<open>Code Block & Current Construction & Pending Construction\<close>
+definition \<open>Filter_Out_Values (T::'a set) (T'::'a set) \<equiv> Trueprop (\<^bold>s\<^bold>u\<^bold>b\<^bold>t\<^bold>y\<^bold>p\<^bold>e T \<longmapsto> T')\<close>
+definition \<open>Assertion_Level_SubType_Reasoning T \<equiv> Trueprop T\<close>
+
+subsection \<open>Current Construction & Pending Construction\<close>
 
 (* syntax "_codeblock_exp_" :: "idt \<Rightarrow> logic \<Rightarrow> logic \<Rightarrow> bool"  ("(2\<^bold>c\<^bold>o\<^bold>d\<^bold>e\<^bold>b\<^bold>l\<^bold>o\<^bold>c\<^bold>k _/  \<^bold>a\<^bold>s '\<open>_'\<close>/ \<^bold>f\<^bold>o\<^bold>r \<^bold>a\<^bold>r\<^bold>g\<^bold>u\<^bold>m\<^bold>e\<^bold>n\<^bold>t\<^bold>s '\<open>_'\<close>)" [100,0,0] 3)
 syntax "_codeblock_" :: "idt \<Rightarrow> logic \<Rightarrow> bool" ("\<^bold>c\<^bold>o\<^bold>d\<^bold>e\<^bold>b\<^bold>l\<^bold>o\<^bold>c\<^bold>k _ \<^bold>f\<^bold>o\<^bold>r \<^bold>a\<^bold>r\<^bold>g\<^bold>u\<^bold>m\<^bold>e\<^bold>n\<^bold>t\<^bold>s '\<open>_'\<close>" [100,0] 3) *)
@@ -141,8 +378,23 @@ lemma \<phi>rename_proc_with_goal:
   \<open>f \<equiv> f' \<Longrightarrow> \<^bold>p\<^bold>r\<^bold>o\<^bold>c f' \<lbrace> U \<longmapsto> \<R> \<^bold>t\<^bold>h\<^bold>r\<^bold>o\<^bold>w\<^bold>s E \<rbrace> \<^bold>@\<^bold>G\<^bold>O\<^bold>A\<^bold>L G \<Longrightarrow> \<^bold>p\<^bold>r\<^bold>o\<^bold>c f \<lbrace> U \<longmapsto> \<R> \<^bold>t\<^bold>h\<^bold>r\<^bold>o\<^bold>w\<^bold>s E \<rbrace> \<^bold>@\<^bold>G\<^bold>O\<^bold>A\<^bold>L G\<close>
   unfolding GOAL_CTXT_def using \<phi>rename_proc .
 
-
 end
+
+paragraph \<open>Simplification in the Programming\<close>
+
+
+lemma (in std) [simp]:
+  "(\<^bold>c\<^bold>u\<^bold>r\<^bold>r\<^bold>e\<^bold>n\<^bold>t s [H] \<^bold>r\<^bold>e\<^bold>s\<^bold>u\<^bold>l\<^bold>t\<^bold>s \<^bold>i\<^bold>n T \<^bold>s\<^bold>u\<^bold>b\<^bold>j P) \<longleftrightarrow> (\<^bold>c\<^bold>u\<^bold>r\<^bold>r\<^bold>e\<^bold>n\<^bold>t s [H] \<^bold>r\<^bold>e\<^bold>s\<^bold>u\<^bold>l\<^bold>t\<^bold>s \<^bold>i\<^bold>n T) \<and> P"
+  unfolding CurrentConstruction_def by (simp_all add: \<phi>expns pair_All) blast
+
+lemma (in std) [simp]:
+  "((\<^bold>c\<^bold>u\<^bold>r\<^bold>r\<^bold>e\<^bold>n\<^bold>t s [H] \<^bold>r\<^bold>e\<^bold>s\<^bold>u\<^bold>l\<^bold>t\<^bold>s \<^bold>i\<^bold>n T) \<and> B) \<and> C \<longleftrightarrow> (\<^bold>c\<^bold>u\<^bold>r\<^bold>r\<^bold>e\<^bold>n\<^bold>t s [H] \<^bold>r\<^bold>e\<^bold>s\<^bold>u\<^bold>l\<^bold>t\<^bold>s \<^bold>i\<^bold>n T) \<and> (B \<and> C)"
+  by simp
+
+lemma (in std) \<phi>ExTyp_strip:
+  "(\<^bold>c\<^bold>u\<^bold>r\<^bold>r\<^bold>e\<^bold>n\<^bold>t p [H] \<^bold>r\<^bold>e\<^bold>s\<^bold>u\<^bold>l\<^bold>t\<^bold>s \<^bold>i\<^bold>n (ExSet T)) \<equiv> (\<exists>c. \<^bold>c\<^bold>u\<^bold>r\<^bold>r\<^bold>e\<^bold>n\<^bold>t p [H] \<^bold>r\<^bold>e\<^bold>s\<^bold>u\<^bold>l\<^bold>t\<^bold>s \<^bold>i\<^bold>n T c)"
+  unfolding CurrentConstruction_def atomize_eq by (simp_all add: \<phi>expns pair_All) blast
+
 
 
 subsection \<open>Antecedents of Reasoning - Part I\<close>
@@ -273,6 +525,7 @@ proof fix x assume "(\<And>x. PROP P x)" then show "PROP P (tag x)" .
 next fix x :: "'a <named> 'b" assume "(\<And>x. PROP P (tag x))" from \<open>PROP P (tag (case x of tag x \<Rightarrow> x))\<close> show "PROP P x" by simp
 qed
 
+lemma named_ExSet: "(ExSet T) = (\<exists>*c. T (tag c) )" by (auto simp add: named_exists \<phi>expns)
 
 subsubsection \<open>Rename \<lambda>-Abstraction\<close>
 
@@ -353,247 +606,6 @@ ML_file "library/reasoners.ML"
 
 
 
-section \<open>\<phi>-Type\<close>
-
-type_synonym ('concrete,'abstract) \<phi> = " 'abstract \<Rightarrow> 'concrete set "
-
-
-subsubsection \<open>Definitions\<close>
-
-definition \<phi>Type :: "'b \<Rightarrow> ('a,'b) \<phi> \<Rightarrow> 'a set" (infix "\<Ztypecolon>" 20) where " (x \<Ztypecolon> T) = (T x)"
-
-lemma typing_inhabited: "p \<in> (x \<Ztypecolon> T) \<Longrightarrow> Inhabited (x \<Ztypecolon> T)"
-  unfolding Inhabited_def \<phi>Type_def by blast
-
-lemma \<phi>Type_eqI:
-  \<open>(\<forall>x p. p \<in> (x \<Ztypecolon> a) \<longleftrightarrow> p \<in> (x \<Ztypecolon> b)) \<Longrightarrow> a = b\<close>
-  unfolding \<phi>Type_def by blast
-
-
-
-paragraph \<open>Syntax\<close>
-
-abbreviation (in std) COMMA
-  :: \<open>('FIC_N,'FIC) assn \<Rightarrow> ('FIC_N,'FIC) assn \<Rightarrow> ('FIC_N,'FIC) assn\<close> (infixl "\<heavy_comma>" 13)
-  where \<open>COMMA \<equiv> (*)\<close>
-
-(*
-setup \<open>(Sign.add_trrules (let open Ast 
-      fun nuty x y = Appl [Constant \<^const_syntax>\<open>\<phi>Type\<close>, Variable x, Variable y]
-      fun wrap_ele tm = Appl [Constant \<^const_syntax>\<open>Ele\<close>, tm]
-      fun wrap_nuty x y = wrap_ele (nuty x y)
-    in [
-      Syntax.Parse_Print_Rule (
-        Appl [Constant "\<^const>local.COMMA", nuty "x" "T", Variable "U"],
-        Appl [Constant "\<^const>local.COMMA", wrap_nuty "x" "T", Variable "U"]),
-      Syntax.Parse_Print_Rule (
-        Appl [Constant "\<^const>local.COMMA", Variable "U", nuty "x" "T"],
-        Appl [Constant "\<^const>local.COMMA", Variable "U", wrap_nuty "x" "T"]),
-      Syntax.Parse_Print_Rule (
-        Appl [Constant "\<^const>local.\<phi>Procedure", Variable "f", nuty "x" "T", Variable "U"],
-        Appl [Constant "\<^const>local.\<phi>Procedure", Variable "f", wrap_nuty "x" "T", Variable "U"]),
-      Syntax.Parse_Print_Rule (
-        Appl [Constant "\<^const>local.\<phi>Procedure", Variable "f", Variable "U", nuty "x" "T"],
-        Appl [Constant "\<^const>local.\<phi>Procedure", Variable "f", Variable "U", wrap_nuty "x" "T"]),
-      Syntax.Parse_Print_Rule (
-        Appl [Constant "\<^const>local.\<phi>Procedure_no_exception", Variable "f", nuty "x" "T", Variable "U"],
-        Appl [Constant "\<^const>local.\<phi>Procedure_no_exception", Variable "f", wrap_nuty "x" "T", Variable "U"]),
-      Syntax.Parse_Print_Rule (
-        Appl [Constant "\<^const>local.\<phi>Procedure_no_exception", Variable "f", Variable "U", nuty "x" "T"],
-        Appl [Constant "\<^const>local.\<phi>Procedure_no_exception", Variable "f", Variable "U", wrap_nuty "x" "T"]),
-      Syntax.Parse_Print_Rule (
-        Appl [Constant "\<^const>local.CurrentConstruction", Variable "s", Variable "R", nuty "x" "T"],
-        Appl [Constant "\<^const>local.CurrentConstruction", Variable "s", Variable "R", wrap_nuty "x" "T"]),
-      Syntax.Parse_Print_Rule (
-        Appl [Constant "\<^const>local.PendingConstruction", Variable "f", Variable "s", Variable "R", nuty "x" "T"],
-        Appl [Constant "\<^const>local.PendingConstruction", Variable "f", Variable "s", Variable "R", wrap_nuty "x" "T"])
-  ] end))\<close>
-*)
-
-subsubsection \<open>Properties\<close>
-
-context std_sem begin
-
-definition \<phi>SemType :: "'VAL set \<Rightarrow> 'TY \<Rightarrow> bool"
-  where [\<phi>def]: \<open>\<phi>SemType S TY \<longleftrightarrow> S \<subseteq> Well_Type TY\<close>
-
-abbreviation \<phi>\<phi>SemType :: "('VAL, 'a) \<phi> \<Rightarrow> 'TY \<Rightarrow> bool"
-  where \<open>\<phi>\<phi>SemType T TY \<equiv> (\<forall>x. \<phi>SemType (x \<Ztypecolon> T) TY)\<close>
-
-definition \<phi>Zero :: "'TY \<Rightarrow> ('VAL,'a) \<phi> \<Rightarrow> 'a \<Rightarrow> bool"
-  where [\<phi>def]: "\<phi>Zero ty T x \<longleftrightarrow> Zero ty \<in> (x \<Ztypecolon> T)"
-
-definition \<phi>Equal :: "('VAL,'a) \<phi> \<Rightarrow> ('a \<Rightarrow> 'a \<Rightarrow> bool) \<Rightarrow> ('a \<Rightarrow> 'a \<Rightarrow> bool) \<Rightarrow> bool"
-  where [\<phi>def]: "\<phi>Equal T can_eq eq \<longleftrightarrow> (\<forall>p1 p2 x1 x2 res.
-    can_eq x1 x2 \<and> p1 \<in> (x1 \<Ztypecolon> T) \<and> p2 \<in> (x2 \<Ztypecolon> T)
-      \<longrightarrow> Can_EqCompare res p1 p2 \<and> (EqCompare p1 p2 = eq x1 x2))"
-
-end
-
-definition Subty :: " 'a set \<Rightarrow> 'a set \<Rightarrow> bool \<Rightarrow> bool " ("(2\<^bold>s\<^bold>u\<^bold>b\<^bold>t\<^bold>y\<^bold>p\<^bold>e _/ \<longmapsto> _/ \<^bold>w\<^bold>i\<^bold>t\<^bold>h _)" [13,13,13] 12)
-  where "(\<^bold>s\<^bold>u\<^bold>b\<^bold>t\<^bold>y\<^bold>p\<^bold>e A \<longmapsto> B \<^bold>w\<^bold>i\<^bold>t\<^bold>h P) \<longleftrightarrow> (\<forall>v. v \<in> A \<longrightarrow> v \<in> B \<and> P)"
-
-subsubsection \<open>Subjection\<close>
-
-definition Subjection :: " 'p set \<Rightarrow> bool \<Rightarrow> 'p set " (infixl "\<^bold>s\<^bold>u\<^bold>b\<^bold>j" 13)
-  where " (T \<^bold>s\<^bold>u\<^bold>b\<^bold>j P) = {p. p \<in> T \<and> P}"
-
-lemma Subjection_expn[\<phi>expns]:
-  "p \<in> (T \<^bold>s\<^bold>u\<^bold>b\<^bold>j P) \<longleftrightarrow> p \<in> T \<and> P"
-  unfolding Subjection_def by simp
-
-lemma Subjection_inhabited[elim!,\<phi>reason_elim!]:
-  \<open>Inhabited (S \<^bold>s\<^bold>u\<^bold>b\<^bold>j P) \<Longrightarrow> (P \<Longrightarrow> Inhabited S \<Longrightarrow> C) \<Longrightarrow> C\<close>
-  unfolding Inhabited_def by (simp add: \<phi>expns)
-
-lemma [\<phi>reason]:
-  " \<^bold>s\<^bold>u\<^bold>b\<^bold>t\<^bold>y\<^bold>p\<^bold>e T \<longmapsto> T' \<^bold>w\<^bold>i\<^bold>t\<^bold>h P
-\<Longrightarrow> (P \<Longrightarrow> \<^bold>p\<^bold>r\<^bold>e\<^bold>m\<^bold>i\<^bold>s\<^bold>e Q)
-\<Longrightarrow> \<^bold>s\<^bold>u\<^bold>b\<^bold>t\<^bold>y\<^bold>p\<^bold>e T \<longmapsto> T' \<^bold>s\<^bold>u\<^bold>b\<^bold>j Q \<^bold>w\<^bold>i\<^bold>t\<^bold>h P"
-  unfolding Subty_def Premise_def by (simp add: \<phi>expns)
-
-lemma [simp]: "(T \<^bold>s\<^bold>u\<^bold>b\<^bold>j True) = T" by (auto simp add: \<phi>expns)
-(* lemma (in std) [simp]: "(VAL (S \<^bold>s\<^bold>u\<^bold>b\<^bold>j P)) = (VAL S \<^bold>s\<^bold>u\<^bold>b\<^bold>j P)" by (simp add: \<phi>expns set_eq_iff) blast
-lemma (in std) [simp]: "(OBJ (S \<^bold>s\<^bold>u\<^bold>b\<^bold>j P)) = (OBJ S \<^bold>s\<^bold>u\<^bold>b\<^bold>j P)" by (simp add: \<phi>expns set_eq_iff) *)
-
-lemma Subjection_times[simp]:
-  \<open>(S \<^bold>s\<^bold>u\<^bold>b\<^bold>j P) * T = (S * T \<^bold>s\<^bold>u\<^bold>b\<^bold>j P)\<close>
-  \<open>T * (S \<^bold>s\<^bold>u\<^bold>b\<^bold>j P) = (T * S \<^bold>s\<^bold>u\<^bold>b\<^bold>j P)\<close>
-  unfolding Subjection_def times_set_def set_eq_iff by blast+
-
-
-(* declare split_paired_All[simp del] split_paired_Ex[simp del] *)
-
-lemma (in std) Subjection_simp_proc_arg'[simp]:
-  "\<^bold>p\<^bold>r\<^bold>o\<^bold>c f \<lbrace> T \<^bold>s\<^bold>u\<^bold>b\<^bold>j P \<longmapsto> Y \<^bold>t\<^bold>h\<^bold>r\<^bold>o\<^bold>w\<^bold>s E \<rbrace> = (P \<longrightarrow> \<^bold>p\<^bold>r\<^bold>o\<^bold>c f \<lbrace> T \<longmapsto> Y \<^bold>t\<^bold>h\<^bold>r\<^bold>o\<^bold>w\<^bold>s E \<rbrace>)"
-  (* and Subjection_simp_func_arg[simp]: "\<^bold>f\<^bold>u\<^bold>n\<^bold>c f' \<lbrace> T \<and>\<^sup>s P \<longmapsto> Y \<rbrace> = (P \<longrightarrow> \<^bold>f\<^bold>u\<^bold>n\<^bold>c f' \<lbrace> T \<longmapsto> Y \<rbrace>)" *)
-  unfolding \<phi>Procedure_def by (simp add: \<phi>expns) blast
-
-lemmas (in std) Subjection_simp_proc_arg[unfolded atomize_eq[symmetric]] = Subjection_simp_proc_arg'
-
-lemma (in std) [simp]:
-  "(\<^bold>c\<^bold>u\<^bold>r\<^bold>r\<^bold>e\<^bold>n\<^bold>t s [H] \<^bold>r\<^bold>e\<^bold>s\<^bold>u\<^bold>l\<^bold>t\<^bold>s \<^bold>i\<^bold>n T \<^bold>s\<^bold>u\<^bold>b\<^bold>j P) \<longleftrightarrow> (\<^bold>c\<^bold>u\<^bold>r\<^bold>r\<^bold>e\<^bold>n\<^bold>t s [H] \<^bold>r\<^bold>e\<^bold>s\<^bold>u\<^bold>l\<^bold>t\<^bold>s \<^bold>i\<^bold>n T) \<and> P"
-  unfolding CurrentConstruction_def by (simp_all add: \<phi>expns pair_All) blast
-
-lemma (in std) [simp]:
-  "((\<^bold>c\<^bold>u\<^bold>r\<^bold>r\<^bold>e\<^bold>n\<^bold>t s [H] \<^bold>r\<^bold>e\<^bold>s\<^bold>u\<^bold>l\<^bold>t\<^bold>s \<^bold>i\<^bold>n T) \<and> B) \<and> C \<longleftrightarrow> (\<^bold>c\<^bold>u\<^bold>r\<^bold>r\<^bold>e\<^bold>n\<^bold>t s [H] \<^bold>r\<^bold>e\<^bold>s\<^bold>u\<^bold>l\<^bold>t\<^bold>s \<^bold>i\<^bold>n T) \<and> (B \<and> C)"
-  by simp
-
-
-(* ML \<open>Theory.setup (Sign.add_trrules (let open Ast 
-      fun nuty x y = Appl [Constant \<^const_syntax>\<open>\<phi>Type\<close>, Variable x, Variable y]
-      fun wrap_ele tm = Appl [Constant \<^const_syntax>\<open>Ele\<close>, tm]
-      fun wrap_nuty x y = wrap_ele (nuty x y)
-      fun subj x = Appl [Constant \<^const_syntax>\<open>Subjection\<close>, x, Variable "P"]
-    in [
-      Syntax.Parse_Print_Rule (
-        Appl [Constant "\<^const>local.\<phi>Procedure", Variable "f", subj (nuty "x" "T"), Variable "U"],
-        Appl [Constant "\<^const>local.\<phi>Procedure", Variable "f", subj (wrap_nuty "x" "T"), Variable "U"]),
-      Syntax.Parse_Print_Rule (
-        Appl [Constant "\<^const>local.\<phi>Procedure", Variable "f", Variable "U", subj (nuty "x" "T")],
-        Appl [Constant "\<^const>local.\<phi>Procedure", Variable "f", Variable "U", subj (wrap_nuty "x" "T")]),
-      Syntax.Parse_Print_Rule (
-        Appl [Constant "\<^const>local.\<phi>Procedure_no_exception", Variable "f", subj (nuty "x" "T"), Variable "U"],
-        Appl [Constant "\<^const>local.\<phi>Procedure_no_exception", Variable "f", subj (wrap_nuty "x" "T"), Variable "U"]),
-      Syntax.Parse_Print_Rule (
-        Appl [Constant "\<^const>local.\<phi>Procedure_no_exception", Variable "f", Variable "U", subj (nuty "x" "T")],
-        Appl [Constant "\<^const>local.\<phi>Procedure_no_exception", Variable "f", Variable "U", subj (wrap_nuty "x" "T")])
-  ] end))\<close>
-*)
-
-
-subsubsection \<open>Existential Quantification\<close>
-
-definition ExSet :: " ('c \<Rightarrow> 'a set) \<Rightarrow> 'a set" (binder "\<exists>*" 10)
-  where "ExSet S = {p. (\<exists>c. p \<in> S c)}"
-notation ExSet (binder "\<exists>\<^sup>s" 10)
-
-
-lemma [\<phi>expns]: "p \<in> ExSet S \<longleftrightarrow> (\<exists>c. p \<in> S c)" unfolding ExSet_def by simp
-
-syntax
-  "_SetcomprNu" :: "'a \<Rightarrow> idts \<Rightarrow> bool \<Rightarrow> 'a set"  ("_ \<^bold>s\<^bold>u\<^bold>b\<^bold>j/ _./ _" [3,0,4] 3)
-
-translations
-  " X \<^bold>s\<^bold>u\<^bold>b\<^bold>j idts. P " \<rightleftharpoons> "\<exists>* idts. X \<^bold>s\<^bold>u\<^bold>b\<^bold>j P"
-  " X \<^bold>s\<^bold>u\<^bold>b\<^bold>j idts. CONST True " \<rightleftharpoons> "\<exists>* idts. X"
-
-
-(*
-ML \<open>Theory.setup (Sign.add_trrules (let open Ast 
-      fun nuty x y = Appl [Constant \<^const_syntax>\<open>\<phi>Type\<close>, Variable x, Variable y]
-      fun wrap_ele tm = Appl [Constant \<^const_syntax>\<open>Ele\<close>, tm]
-      fun wrap_nuty x y = wrap_ele (nuty x y)
-      fun subj x = Appl [Constant \<^syntax_const>\<open>_SetcomprNu\<close>, x, Variable "idts", Variable "P"]
-    in [
-      Syntax.Parse_Print_Rule (
-        Appl [Constant "\<^const>local.\<phi>Procedure", Variable "f", subj (nuty "x" "T"), Variable "U"],
-        Appl [Constant "\<^const>local.\<phi>Procedure", Variable "f", subj (wrap_nuty "x" "T"), Variable "U"]),
-      Syntax.Parse_Print_Rule (
-        Appl [Constant "\<^const>local.\<phi>Procedure", Variable "f", Variable "U", subj (nuty "x" "T")],
-        Appl [Constant "\<^const>local.\<phi>Procedure", Variable "f", Variable "U", subj (wrap_nuty "x" "T")]),
-      Syntax.Parse_Print_Rule (
-        Appl [Constant "\<^const>local.\<phi>Procedure_no_exception", Variable "f", subj (nuty "x" "T"), Variable "U"],
-        Appl [Constant "\<^const>local.\<phi>Procedure_no_exception", Variable "f", subj (wrap_nuty "x" "T"), Variable "U"]),
-      Syntax.Parse_Print_Rule (
-        Appl [Constant "\<^const>local.\<phi>Procedure_no_exception", Variable "f", Variable "U", subj (nuty "x" "T")],
-        Appl [Constant "\<^const>local.\<phi>Procedure_no_exception", Variable "f", Variable "U", subj (wrap_nuty "x" "T")])
-  ] end))\<close>
-*)
-text (in std)
- \<open>The set of \<phi>-type in an assertion like \<^term>\<open>\<^bold>p\<^bold>r\<^bold>o\<^bold>c f \<lbrace> S x \<^bold>s\<^bold>u\<^bold>b\<^bold>j x. P x \<longmapsto> \<lambda>ret. T x \<^bold>s\<^bold>u\<^bold>b\<^bold>j x. Q x \<rbrace>\<close> is represented
-  by \<^const>\<open>ExSet\<close> and we show a \<phi>-type \<^term>\<open>S x \<^bold>s\<^bold>u\<^bold>b\<^bold>j x. P x\<close> represents actually all concrete values that
-  belongs to \<^term>\<open>S\<close> a set of \<phi>-types (i.e. the union of \<^term>\<open>S\<close>) by following lemma\<close>
-
-lemma " Union { S x |x. P x } = (S x \<^bold>s\<^bold>u\<^bold>b\<^bold>j x. P x) "
-  by (simp add: set_eq_iff \<phi>expns) blast
-
-
-lemma ExSet_pair: "ExSet T = (\<exists>*c1 c2. T (c1,c2) )" by (auto simp add: \<phi>expns)
-lemma named_ExSet: "(ExSet T) = (\<exists>*c. T (tag c) )" by (auto simp add: named_exists \<phi>expns)
-
-(* lemma (in std_sem) [simp]: "p \<in> \<S>  (ExSet T) \<longleftrightarrow> (\<exists>z. p \<in> \<S>  (T z) )" by (cases p, simp_all add: \<phi>expns set_eq_iff)
-lemma (in std_sem) [simp]: "p \<in> !\<S> (ExSet T) \<longleftrightarrow> (\<exists>z. p \<in> !\<S> (T z) )" by (cases p, simp_all add: \<phi>expns set_eq_iff) *)
-(* lemma (in std) [simp]: "(VAL ExSet T) = (\<exists>*c. VAL T c)" by (simp add: \<phi>expns set_eq_iff) blast
-lemma (in std) [simp]: "(OBJ ExSet T) = (\<exists>*c. OBJ T c)" by (simp add: \<phi>expns set_eq_iff) *)
-lemma [simp]: "(ExSet T * R) = (\<exists>* c. T c * R )" by (simp add: \<phi>expns set_eq_iff) blast
-lemma ExSet_times[simp]: "(L * ExSet T) = (\<exists>* c. L * T c)" by (simp add: \<phi>expns set_eq_iff) blast
-
-lemma ExSet_ExSet[simp]:
-  \<open>(X a b \<^bold>s\<^bold>u\<^bold>b\<^bold>j a. P a b \<^bold>s\<^bold>u\<^bold>b\<^bold>j b. Q b) = (X a b \<^bold>s\<^bold>u\<^bold>b\<^bold>j a b. P a b \<and> Q b)\<close>
-  unfolding set_eq_iff by (simp add: \<phi>expns, blast)
-
-lemma ExSet_SubjSet[simp]:
-  \<open>(X b \<^bold>s\<^bold>u\<^bold>b\<^bold>j P b \<^bold>s\<^bold>u\<^bold>b\<^bold>j b. Q b) = (X b \<^bold>s\<^bold>u\<^bold>b\<^bold>j b. P b \<and> Q b)\<close>
-  unfolding set_eq_iff by (simp add: \<phi>expns)
-
-
-lemma (in std) \<phi>ExTyp_strip:
-  "(\<^bold>c\<^bold>u\<^bold>r\<^bold>r\<^bold>e\<^bold>n\<^bold>t p [H] \<^bold>r\<^bold>e\<^bold>s\<^bold>u\<^bold>l\<^bold>t\<^bold>s \<^bold>i\<^bold>n (ExSet T)) \<equiv> (\<exists>c. \<^bold>c\<^bold>u\<^bold>r\<^bold>r\<^bold>e\<^bold>n\<^bold>t p [H] \<^bold>r\<^bold>e\<^bold>s\<^bold>u\<^bold>l\<^bold>t\<^bold>s \<^bold>i\<^bold>n T c)"
-  unfolding CurrentConstruction_def atomize_eq by (simp_all add: \<phi>expns pair_All) blast
-
-lemma [\<phi>reason 200]: "(\<And>c. \<^bold>s\<^bold>u\<^bold>b\<^bold>t\<^bold>y\<^bold>p\<^bold>e T c \<longmapsto> T' \<^bold>w\<^bold>i\<^bold>t\<^bold>h P c) \<Longrightarrow> \<^bold>s\<^bold>u\<^bold>b\<^bold>t\<^bold>y\<^bold>p\<^bold>e (ExSet T) \<longmapsto> T' \<^bold>w\<^bold>i\<^bold>t\<^bold>h (\<exists>c. P c)"
-  unfolding Subty_def by (simp add: \<phi>expns) blast
-
-subsubsection \<open>Simplification & Reasoning\<close>
-
-ML_file \<open>library/NuSimpCongruence.ML\<close>
-
-lemma (in std) \<phi>CONSEQ':
-   "\<^bold>s\<^bold>u\<^bold>b\<^bold>t\<^bold>y\<^bold>p\<^bold>e A' \<longmapsto> A \<^bold>w\<^bold>i\<^bold>t\<^bold>h P1
-\<Longrightarrow> (\<And>x. \<^bold>s\<^bold>u\<^bold>b\<^bold>t\<^bold>y\<^bold>p\<^bold>e B x \<longmapsto> B' x \<^bold>w\<^bold>i\<^bold>t\<^bold>h P2)
-\<Longrightarrow> \<^bold>s\<^bold>u\<^bold>b\<^bold>t\<^bold>y\<^bold>p\<^bold>e E \<longmapsto> E' \<^bold>w\<^bold>i\<^bold>t\<^bold>h P3
-\<Longrightarrow> \<^bold>p\<^bold>r\<^bold>o\<^bold>c f \<lbrace> A  \<longmapsto> B  \<^bold>t\<^bold>h\<^bold>r\<^bold>o\<^bold>w\<^bold>s E  \<rbrace>
-\<Longrightarrow> \<^bold>p\<^bold>r\<^bold>o\<^bold>c f \<lbrace> A' \<longmapsto> B' \<^bold>t\<^bold>h\<^bold>r\<^bold>o\<^bold>w\<^bold>s E' \<rbrace>"
-  unfolding Subty_def
-  by (meson \<phi>CONSEQ subsetI)
-
-lemma (in std) \<phi>CONSEQ'E:
-   "\<^bold>s\<^bold>u\<^bold>b\<^bold>t\<^bold>y\<^bold>p\<^bold>e E \<longmapsto> E' \<^bold>w\<^bold>i\<^bold>t\<^bold>h P3
-\<Longrightarrow> \<^bold>p\<^bold>r\<^bold>o\<^bold>c f \<lbrace> A  \<longmapsto> B  \<^bold>t\<^bold>h\<^bold>r\<^bold>o\<^bold>w\<^bold>s E  \<rbrace>
-\<Longrightarrow> \<^bold>p\<^bold>r\<^bold>o\<^bold>c f \<lbrace> A \<longmapsto> B \<^bold>t\<^bold>h\<^bold>r\<^bold>o\<^bold>w\<^bold>s E' \<rbrace>"
-  unfolding Subty_def
-  by (meson \<phi>CONSEQ subsetI)
 
 
 section \<open>More Features of the Deductive Programming\<close>
@@ -667,6 +679,15 @@ lemma (in std) "\<phi>__final_proc_rewrite__'":
 \<Longrightarrow> \<^bold>p\<^bold>r\<^bold>o\<^bold>c f' \<lbrace> P \<longmapsto> Q \<^bold>t\<^bold>h\<^bold>r\<^bold>o\<^bold>w\<^bold>s E\<rbrace> \<^bold>@\<^bold>G\<^bold>O\<^bold>A\<^bold>L G\<close>
   unfolding Conv_def by simp
 
+subsubsection \<open>Misc\<close>
+
+lemma (in std) "\<phi>__Return_rule__":
+  \<open> \<^bold>s\<^bold>u\<^bold>b\<^bold>t\<^bold>y\<^bold>p\<^bold>e X \<longmapsto> Y \<^bold>w\<^bold>i\<^bold>t\<^bold>h Any
+\<Longrightarrow> \<^bold>p\<^bold>r\<^bold>o\<^bold>c Return (sem_value ()) \<lbrace> X \<longmapsto> \<lambda>_::unit sem_value. Y \<rbrace>\<close>
+  unfolding \<phi>Procedure_def Return_def Subty_def by (simp add: \<phi>expns) blast
+
+
+
 subsection \<open>Ad-hoc Overload\<close>
 
 ML_file \<open>library/applicant.ML\<close>
@@ -682,9 +703,6 @@ attribute_setup \<phi>overload = \<open>Scan.lift (Parse.and_list1 NuApplicant.n
 subsection \<open>Subtype & View Shift\<close>
 
 paragraph \<open>Definitions\<close>
-
-consts SimpleSubty :: " 'a set \<Rightarrow> 'a set \<Rightarrow> bool \<Rightarrow> bool " ("(2\<^bold>s\<^bold>u\<^bold>b\<^bold>t\<^bold>y\<^bold>p\<^bold>e _/ \<longmapsto> _)" [13,13] 12)
-translations "(\<^bold>s\<^bold>u\<^bold>b\<^bold>t\<^bold>y\<^bold>p\<^bold>e A \<longmapsto> B)" == "(\<^bold>s\<^bold>u\<^bold>b\<^bold>t\<^bold>y\<^bold>p\<^bold>e A \<longmapsto> B \<^bold>w\<^bold>i\<^bold>t\<^bold>h CONST True)"
 
 definition (in std) Viewshft :: \<open> ('FIC_N \<Rightarrow> 'FIC) set \<Rightarrow> ('FIC_N \<Rightarrow> 'FIC) set \<Rightarrow> bool \<Rightarrow> bool \<close>
   ("(2\<^bold>v\<^bold>i\<^bold>e\<^bold>w\<^bold>'_\<^bold>s\<^bold>h\<^bold>i\<^bold>f\<^bold>t _/ \<longmapsto> _/ \<^bold>w\<^bold>i\<^bold>t\<^bold>h _)" [13,13,13] 12)
@@ -834,17 +852,6 @@ lemma IntroFrameVar'_Yes:
 
 end
 
-paragraph \<open>Simplify \<open>R\<heavy_comma> 0\<close>\<close>
-
-consts frame_over_zero :: mode
-
-lemma [\<phi>reason 3000 on \<open>\<^bold>s\<^bold>i\<^bold>m\<^bold>p\<^bold>l\<^bold>i\<^bold>f\<^bold>y[frame_over_zero] ?Y : ?R * 0\<close>]:
-  \<open>\<^bold>s\<^bold>i\<^bold>m\<^bold>p\<^bold>l\<^bold>i\<^bold>f\<^bold>y[frame_over_zero] 0 : R * 0\<close> for R :: \<open>'a::times set\<close>
-  unfolding Simplify_def by simp
-
-lemma [\<phi>reason 2000 on \<open>\<^bold>s\<^bold>i\<^bold>m\<^bold>p\<^bold>l\<^bold>i\<^bold>f\<^bold>y[frame_over_zero] ?Y : ?X\<close>]:
-  \<open>\<^bold>s\<^bold>i\<^bold>m\<^bold>p\<^bold>l\<^bold>i\<^bold>f\<^bold>y[frame_over_zero] X : X\<close> for R :: \<open>'a::times set\<close>
-  unfolding Simplify_def by simp
 
 subsubsection \<open>Fix\<close>
 
@@ -1259,16 +1266,14 @@ lemma \<phi>apply_subtyping_fully[\<phi>reason on \<open>
       (Trueprop (\<^bold>c\<^bold>u\<^bold>r\<^bold>r\<^bold>e\<^bold>n\<^bold>t ?blk [?RR] \<^bold>r\<^bold>e\<^bold>s\<^bold>u\<^bold>l\<^bold>t\<^bold>s \<^bold>i\<^bold>n ?S)) ?Result
 \<close>]:
   "IntroFrameVar R S'' S' T T'
-\<Longrightarrow> SUBGOAL TOP_GOAL G
-\<Longrightarrow> \<^bold>s\<^bold>u\<^bold>b\<^bold>t\<^bold>y\<^bold>p\<^bold>e S \<longmapsto> \<blangle> S'' \<brangle> \<^bold>w\<^bold>i\<^bold>t\<^bold>h Any  \<^bold>@\<^bold>G\<^bold>O\<^bold>A\<^bold>L G
-\<Longrightarrow> SOLVE_SUBGOAL G
+\<Longrightarrow> PROP Assertion_Level_SubType_Reasoning (\<^bold>s\<^bold>u\<^bold>b\<^bold>t\<^bold>y\<^bold>p\<^bold>e S \<longmapsto> S'' \<^bold>w\<^bold>i\<^bold>t\<^bold>h Any)
 \<Longrightarrow> PROP \<phi>Application_Success
 \<Longrightarrow> \<^bold>o\<^bold>b\<^bold>l\<^bold>i\<^bold>g\<^bold>a\<^bold>t\<^bold>i\<^bold>o\<^bold>n True
 \<Longrightarrow> PROP \<phi>Application_Method (Trueprop (\<^bold>s\<^bold>u\<^bold>b\<^bold>t\<^bold>y\<^bold>p\<^bold>e S' \<longmapsto> T' \<^bold>w\<^bold>i\<^bold>t\<^bold>h P))
       (Trueprop (\<^bold>c\<^bold>u\<^bold>r\<^bold>r\<^bold>e\<^bold>n\<^bold>t blk [RR] \<^bold>r\<^bold>e\<^bold>s\<^bold>u\<^bold>l\<^bold>t\<^bold>s \<^bold>i\<^bold>n S))
       (Trueprop ((\<^bold>c\<^bold>u\<^bold>r\<^bold>r\<^bold>e\<^bold>n\<^bold>t blk [RR] \<^bold>r\<^bold>e\<^bold>s\<^bold>u\<^bold>l\<^bold>t\<^bold>s \<^bold>i\<^bold>n T) \<and> P))"
   unfolding IntroFrameVar_def \<phi>Application_Method_def \<phi>Application_def
-    GOAL_CTXT_def FOCUS_TAG_def
+    GOAL_CTXT_def FOCUS_TAG_def Assertion_Level_SubType_Reasoning_def
   using "\<phi>cast_P" \<phi>cast_intro_frame
   by (metis (no_types, lifting))
 
@@ -1347,19 +1352,22 @@ lemma \<phi>apply_proc_fully[\<phi>reason on
             (Trueprop (\<^bold>c\<^bold>u\<^bold>r\<^bold>r\<^bold>e\<^bold>n\<^bold>t ?blk [?RR] \<^bold>r\<^bold>e\<^bold>s\<^bold>u\<^bold>l\<^bold>t\<^bold>s \<^bold>i\<^bold>n ?S)) ?Result\<close>
 ]:
   \<open> IntroFrameVar' R S'' S' T T' E'' E'
-\<Longrightarrow> SUBGOAL TOP_GOAL G
-\<Longrightarrow> \<^bold>s\<^bold>u\<^bold>b\<^bold>t\<^bold>y\<^bold>p\<^bold>e S \<longmapsto> \<blangle> S'' \<brangle> \<^bold>w\<^bold>i\<^bold>t\<^bold>h P  \<^bold>@\<^bold>G\<^bold>O\<^bold>A\<^bold>L G
-\<Longrightarrow> SOLVE_SUBGOAL G
-\<Longrightarrow> \<^bold>s\<^bold>i\<^bold>m\<^bold>p\<^bold>l\<^bold>i\<^bold>f\<^bold>y[frame_over_zero] E : E''
+\<Longrightarrow> PROP Assertion_Level_SubType_Reasoning (\<^bold>s\<^bold>u\<^bold>b\<^bold>t\<^bold>y\<^bold>p\<^bold>e S \<longmapsto> S'' \<^bold>w\<^bold>i\<^bold>t\<^bold>h P)
+\<Longrightarrow> PROP Filter_Out_Values E'' E
 \<Longrightarrow> PROP \<phi>Application_Success
 \<Longrightarrow> \<^bold>o\<^bold>b\<^bold>l\<^bold>i\<^bold>g\<^bold>a\<^bold>t\<^bold>i\<^bold>o\<^bold>n True
 \<Longrightarrow> PROP \<phi>Application_Method (Trueprop (\<^bold>p\<^bold>r\<^bold>o\<^bold>c f \<lbrace> S' \<longmapsto> T' \<^bold>t\<^bold>h\<^bold>r\<^bold>o\<^bold>w\<^bold>s E' \<rbrace>))
     (Trueprop (\<^bold>c\<^bold>u\<^bold>r\<^bold>r\<^bold>e\<^bold>n\<^bold>t blk [RR] \<^bold>r\<^bold>e\<^bold>s\<^bold>u\<^bold>l\<^bold>t\<^bold>s \<^bold>i\<^bold>n S))
     (Trueprop (\<^bold>p\<^bold>e\<^bold>n\<^bold>d\<^bold>i\<^bold>n\<^bold>g f \<^bold>o\<^bold>n blk [RR] \<^bold>r\<^bold>e\<^bold>s\<^bold>u\<^bold>l\<^bold>t\<^bold>s \<^bold>i\<^bold>n T \<^bold>t\<^bold>h\<^bold>r\<^bold>o\<^bold>w\<^bold>s E))\<close>
   unfolding \<phi>Application_Method_def \<phi>Application_def IntroFrameVar'_def
-    GOAL_CTXT_def FOCUS_TAG_def Simplify_def
-  using "\<phi>cast" \<phi>apply_proc \<phi>frame[where R=R]
-  by (metis \<phi>CONSEQ' \<phi>frame cast_id)
+    GOAL_CTXT_def FOCUS_TAG_def Simplify_def Assertion_Level_SubType_Reasoning_def
+    Filter_Out_Values_def
+  subgoal premises prems
+    apply (simp only: prems(1))
+    using \<phi>apply_proc[OF \<open>\<^bold>c\<^bold>u\<^bold>r\<^bold>r\<^bold>e\<^bold>n\<^bold>t _ [_] \<^bold>r\<^bold>e\<^bold>s\<^bold>u\<^bold>l\<^bold>t\<^bold>s \<^bold>i\<^bold>n _\<close>,
+          OF \<open>\<^bold>p\<^bold>r\<^bold>o\<^bold>c _ \<lbrace> _ \<longmapsto> _ \<^bold>t\<^bold>h\<^bold>r\<^bold>o\<^bold>w\<^bold>s _ \<rbrace>\<close>[THEN \<phi>frame[where R=R],
+              THEN \<phi>CONSEQ'[OF \<open>\<^bold>s\<^bold>u\<^bold>b\<^bold>t\<^bold>y\<^bold>p\<^bold>e S \<longmapsto> S'' \<^bold>w\<^bold>i\<^bold>t\<^bold>h P\<close>, OF cast_id, OF \<open>\<^bold>s\<^bold>u\<^bold>b\<^bold>t\<^bold>y\<^bold>p\<^bold>e E'' \<longmapsto> E\<close>,
+                simplified prems(1)]]] . .
 
 end
 
@@ -1418,17 +1426,12 @@ lemma (in std) [\<phi>reason 1200 on \<open>
   PROP \<phi>Application_Conv (Trueprop (\<^bold>p\<^bold>r\<^bold>o\<^bold>c ?f \<lbrace> ?X \<longmapsto> ?Y \<^bold>t\<^bold>h\<^bold>r\<^bold>o\<^bold>w\<^bold>s ?E \<rbrace>)) (Trueprop (\<^bold>p\<^bold>r\<^bold>o\<^bold>c ?f' \<lbrace> ?X' \<longmapsto> ?Y' \<^bold>t\<^bold>h\<^bold>r\<^bold>o\<^bold>w\<^bold>s ?E' \<rbrace>))
 \<close>]:
   \<open> Exhaustive_Abstract f f'
-\<Longrightarrow> SUBGOAL TOP_GOAL G1
-\<Longrightarrow> \<^bold>s\<^bold>u\<^bold>b\<^bold>t\<^bold>y\<^bold>p\<^bold>e X' \<longmapsto> \<blangle> X \<brangle> \<^bold>w\<^bold>i\<^bold>t\<^bold>h Any1  \<^bold>@\<^bold>G\<^bold>O\<^bold>A\<^bold>L G1
-\<Longrightarrow> SOLVE_SUBGOAL G1
-\<Longrightarrow> SUBGOAL TOP_GOAL G2
-\<Longrightarrow> (\<And>ret. \<^bold>s\<^bold>u\<^bold>b\<^bold>t\<^bold>y\<^bold>p\<^bold>e Y ret \<longmapsto> \<blangle> Y' ret \<brangle> \<^bold>w\<^bold>i\<^bold>t\<^bold>h Any2  \<^bold>@\<^bold>G\<^bold>O\<^bold>A\<^bold>L G2)
-\<Longrightarrow> SOLVE_SUBGOAL G2
-\<Longrightarrow> SUBGOAL TOP_GOAL G3
-\<Longrightarrow> \<^bold>s\<^bold>u\<^bold>b\<^bold>t\<^bold>y\<^bold>p\<^bold>e E  \<longmapsto> \<blangle> E' \<brangle> \<^bold>w\<^bold>i\<^bold>t\<^bold>h Any3  \<^bold>@\<^bold>G\<^bold>O\<^bold>A\<^bold>L G3
-\<Longrightarrow> SOLVE_SUBGOAL G3
+\<Longrightarrow> PROP Assertion_Level_SubType_Reasoning (\<^bold>s\<^bold>u\<^bold>b\<^bold>t\<^bold>y\<^bold>p\<^bold>e X' \<longmapsto> X \<^bold>w\<^bold>i\<^bold>t\<^bold>h Any1)
+\<Longrightarrow> (\<And>ret. PROP Assertion_Level_SubType_Reasoning (\<^bold>s\<^bold>u\<^bold>b\<^bold>t\<^bold>y\<^bold>p\<^bold>e Y ret \<longmapsto> Y' ret \<^bold>w\<^bold>i\<^bold>t\<^bold>h Any2))
+\<Longrightarrow> PROP Assertion_Level_SubType_Reasoning (\<^bold>s\<^bold>u\<^bold>b\<^bold>t\<^bold>y\<^bold>p\<^bold>e E  \<longmapsto> E' \<^bold>w\<^bold>i\<^bold>t\<^bold>h Any3)
 \<Longrightarrow> PROP \<phi>Application_Conv (Trueprop (\<^bold>p\<^bold>r\<^bold>o\<^bold>c f \<lbrace> X \<longmapsto> Y \<^bold>t\<^bold>h\<^bold>r\<^bold>o\<^bold>w\<^bold>s E \<rbrace>)) (Trueprop (\<^bold>p\<^bold>r\<^bold>o\<^bold>c f' \<lbrace> X' \<longmapsto> Y' \<^bold>t\<^bold>h\<^bold>r\<^bold>o\<^bold>w\<^bold>s E' \<rbrace>))\<close>
   unfolding \<phi>Application_Conv_def Exhaustive_Abstract_def GOAL_CTXT_def FOCUS_TAG_def
+    Assertion_Level_SubType_Reasoning_def
   using \<phi>CONSEQ' by blast
 
 
@@ -1813,6 +1816,22 @@ simproc_setup (in std) Val_simp_cong ("x \<Ztypecolon> Val v T") = \<open>
   K (NuSimpCong.simproc @{thm Val_simp_cong[folded atomize_eq]})
 \<close>
 
+subsubsection \<open>Synthesis\<close>
+
+lemma (in std) [\<phi>reason 2000 on \<open>Synthesis_Parse (?raw::'VAL sem_value) ?Y\<close>]:
+  \<open>Synthesis_Parse raw (\<lambda>_. x \<Ztypecolon> Val raw T)\<close>
+  unfolding Synthesis_Parse_def ..
+
+lemma (in std) [\<phi>reason 1200
+    on \<open>\<^bold>p\<^bold>r\<^bold>o\<^bold>c ?f \<lbrace> ?X \<longmapsto> \<lambda>ret. ?R\<heavy_comma> SYNTHESIS ?x \<Ztypecolon> Val ?raw ?T \<^bold>t\<^bold>h\<^bold>r\<^bold>o\<^bold>w\<^bold>s ?E \<rbrace> \<^bold>@\<^bold>G\<^bold>O\<^bold>A\<^bold>L ?G\<close>
+]:
+  \<open> PROP Assertion_Level_SubType_Reasoning
+      (\<^bold>s\<^bold>u\<^bold>b\<^bold>t\<^bold>y\<^bold>p\<^bold>e X \<longmapsto> R\<heavy_comma> SYNTHESIS x \<Ztypecolon> Val raw T \<^bold>w\<^bold>i\<^bold>t\<^bold>h Any)
+\<Longrightarrow> \<^bold>p\<^bold>r\<^bold>o\<^bold>c Return (sem_value ()) \<lbrace> X \<longmapsto> \<lambda>_::unit sem_value. R\<heavy_comma> SYNTHESIS x \<Ztypecolon> Val raw T \<rbrace> \<^bold>@\<^bold>G\<^bold>O\<^bold>A\<^bold>L G\<close>
+  unfolding Assertion_Level_SubType_Reasoning_def GOAL_CTXT_def
+  by (rule "\<phi>__Return_rule__")
+
+
 
 subsection \<open>Representative Type Tagging\<close>
 
@@ -1954,20 +1973,22 @@ subsection \<open>General Rules & Tools\<close>
 
 lemma (in std) "_\<phi>cast_internal_rule_":
   " \<^bold>c\<^bold>u\<^bold>r\<^bold>r\<^bold>e\<^bold>n\<^bold>t blk [H] \<^bold>r\<^bold>e\<^bold>s\<^bold>u\<^bold>l\<^bold>t\<^bold>s \<^bold>i\<^bold>n T
-\<Longrightarrow> \<^bold>s\<^bold>u\<^bold>b\<^bold>t\<^bold>y\<^bold>p\<^bold>e T \<longmapsto> \<blangle> T' \<brangle> \<^bold>w\<^bold>i\<^bold>t\<^bold>h Any  \<^bold>@\<^bold>G\<^bold>O\<^bold>A\<^bold>L TOP_GOAL
+\<Longrightarrow> PROP Assertion_Level_SubType_Reasoning (\<^bold>s\<^bold>u\<^bold>b\<^bold>t\<^bold>y\<^bold>p\<^bold>e T \<longmapsto> T' \<^bold>w\<^bold>i\<^bold>t\<^bold>h Any)
 \<Longrightarrow> \<r>Success
 \<Longrightarrow> \<^bold>o\<^bold>b\<^bold>l\<^bold>i\<^bold>g\<^bold>a\<^bold>t\<^bold>i\<^bold>o\<^bold>n True
 \<Longrightarrow> \<^bold>c\<^bold>u\<^bold>r\<^bold>r\<^bold>e\<^bold>n\<^bold>t blk [H] \<^bold>r\<^bold>e\<^bold>s\<^bold>u\<^bold>l\<^bold>t\<^bold>s \<^bold>i\<^bold>n T'"
   unfolding CurrentConstruction_def GOAL_CTXT_def Subty_def FOCUS_TAG_def
+    Assertion_Level_SubType_Reasoning_def
   by (simp_all add: pair_All \<phi>expns) blast
 
 lemma (in std) "_\<phi>cast_internal_rule_'":
   " \<^bold>p\<^bold>e\<^bold>n\<^bold>d\<^bold>i\<^bold>n\<^bold>g f \<^bold>o\<^bold>n blk [H] \<^bold>r\<^bold>e\<^bold>s\<^bold>u\<^bold>l\<^bold>t\<^bold>s \<^bold>i\<^bold>n T \<^bold>t\<^bold>h\<^bold>r\<^bold>o\<^bold>w\<^bold>s E
-\<Longrightarrow> (\<And>v. \<^bold>s\<^bold>u\<^bold>b\<^bold>t\<^bold>y\<^bold>p\<^bold>e T v \<longmapsto> \<blangle> T' v \<brangle> \<^bold>w\<^bold>i\<^bold>t\<^bold>h Any  \<^bold>@\<^bold>G\<^bold>O\<^bold>A\<^bold>L TOP_GOAL)
+\<Longrightarrow> (\<And>v. PROP Assertion_Level_SubType_Reasoning (\<^bold>s\<^bold>u\<^bold>b\<^bold>t\<^bold>y\<^bold>p\<^bold>e T v \<longmapsto> T' v \<^bold>w\<^bold>i\<^bold>t\<^bold>h Any))
 \<Longrightarrow> \<r>Success
 \<Longrightarrow> \<^bold>o\<^bold>b\<^bold>l\<^bold>i\<^bold>g\<^bold>a\<^bold>t\<^bold>i\<^bold>o\<^bold>n True
 \<Longrightarrow> \<^bold>p\<^bold>e\<^bold>n\<^bold>d\<^bold>i\<^bold>n\<^bold>g f \<^bold>o\<^bold>n blk [H] \<^bold>r\<^bold>e\<^bold>s\<^bold>u\<^bold>l\<^bold>t\<^bold>s \<^bold>i\<^bold>n T' \<^bold>t\<^bold>h\<^bold>r\<^bold>o\<^bold>w\<^bold>s E"
   unfolding FOCUS_TAG_def Subty_def PendingConstruction_def bind_def GOAL_CTXT_def
+    Assertion_Level_SubType_Reasoning_def
   by (auto simp add: \<phi>expns LooseStateTy_expn') blast+
 
 
@@ -1982,6 +2003,21 @@ lemma (in std) [\<phi>reason 2000 on \<open>\<^bold>s\<^bold>u\<^bold>b\<^bold>t
   \<open> \<^bold>s\<^bold>u\<^bold>b\<^bold>t\<^bold>y\<^bold>p\<^bold>e X \<longmapsto> Y \<^bold>w\<^bold>i\<^bold>t\<^bold>h P
 \<Longrightarrow> \<^bold>s\<^bold>u\<^bold>b\<^bold>t\<^bold>y\<^bold>p\<^bold>e OBJ X \<longmapsto> OBJ Y \<^bold>w\<^bold>i\<^bold>t\<^bold>h P\<close>
   unfolding Subty_def by (simp add: \<phi>expns, blast) *)
+
+
+subsubsection \<open>General Simplification for Assertions\<close>
+
+named_theorems assertion_simps
+
+consts assertion_simplification :: mode
+
+\<phi>reasoner assertion_simplification 1200
+  (conclusion \<open>Simplify assertion_simplification ?X' ?X\<close>)
+  = ((simp only: assertion_simps)?, rule Simplify_I)
+
+lemmas [assertion_simps] =
+  mult_zero_right mult_zero_left mult_1_right mult_1_left add_0_right add_0_left
+
 
 
 subsubsection \<open>Case Analysis\<close>
@@ -2027,7 +2063,7 @@ lemma [\<phi>reason 1000]: "SameNuTy A A" \<comment> \<open>The fallback\<close>
   unfolding SameNuTy_def ..
 
 
-subsection \<open>Assertion Level Sub-type Reasoning\<close>
+subsection \<open>Assertion Level Sub-Type Reasoning\<close>
 
 text \<open>This is a decision procedure reasoning the entailment between assertions.
   It recognizes \<phi>-Types specifying the same object and reduce the goal of assertion entailment
@@ -2044,7 +2080,32 @@ lemmas cast_def = GOAL_CTXT_def FOCUS_TAG_def Subty_def
   "\<^bold>s\<^bold>u\<^bold>b\<^bold>t\<^bold>y\<^bold>p\<^bold>e L * H \<longmapsto> L * H \<^bold>d\<^bold>u\<^bold>a\<^bold>l L * h\<^sub>m \<Ztypecolon> \<blangle> H\<^sub>m \<brangle> \<longmapsto> L * h\<^sub>m \<Ztypecolon> H\<^sub>m \<brangle>"
   unfolding Heap_Subty_Goal_def using cast_dual_id . *)
 
-subsubsection \<open>Identity Subty\<close>
+text \<open>Priority Convention:
+\<^item> 4000: Termination
+\<^item> 3000: Shortcuts like zero
+\<^item> 2000: The framework of step-by-step searching
+\<^item> 2100: Prior rules for specific patterns in the step-by-step searching
+\<^item> 2300: Termination of the step-by-step searching
+\<^item> \<le> 1999: Rules for search specific object like value, variable, etc.
+\<close>
+
+subsubsection \<open>Initialization\<close>
+
+lemma [\<phi>reason 2000]:
+  \<open> Simplify assertion_simplification X' X
+\<Longrightarrow> Simplify assertion_simplification Y' Y
+\<Longrightarrow> SUBGOAL TOP_GOAL G
+\<Longrightarrow> \<^bold>s\<^bold>u\<^bold>b\<^bold>t\<^bold>y\<^bold>p\<^bold>e X' \<longmapsto> \<blangle> Y' \<brangle> \<^bold>w\<^bold>i\<^bold>t\<^bold>h P \<^bold>@\<^bold>G\<^bold>O\<^bold>A\<^bold>L G
+\<Longrightarrow> SOLVE_SUBGOAL G
+\<Longrightarrow> PROP Assertion_Level_SubType_Reasoning (\<^bold>s\<^bold>u\<^bold>b\<^bold>t\<^bold>y\<^bold>p\<^bold>e X \<longmapsto> Y \<^bold>w\<^bold>i\<^bold>t\<^bold>h P)\<close>
+  unfolding Assertion_Level_SubType_Reasoning_def Simplify_def FOCUS_TAG_def
+  by simp
+
+lemma [\<phi>reason 2100 on \<open>PROP Assertion_Level_SubType_Reasoning (\<^bold>s\<^bold>u\<^bold>b\<^bold>t\<^bold>y\<^bold>p\<^bold>e ?X \<longmapsto> ?var_Y \<^bold>w\<^bold>i\<^bold>t\<^bold>h ?P)\<close>]:
+  \<open>PROP Assertion_Level_SubType_Reasoning (\<^bold>s\<^bold>u\<^bold>b\<^bold>t\<^bold>y\<^bold>p\<^bold>e X \<longmapsto> X)\<close>
+  unfolding Assertion_Level_SubType_Reasoning_def using cast_id .
+
+subsubsection \<open>Termination\<close>
 
 lemma [\<phi>reason 4000 on \<open>\<^bold>s\<^bold>u\<^bold>b\<^bold>t\<^bold>y\<^bold>p\<^bold>e ?H \<longmapsto> \<blangle> ?H2 \<brangle> \<^bold>w\<^bold>i\<^bold>t\<^bold>h ?P \<^bold>@\<^bold>G\<^bold>O\<^bold>A\<^bold>L ?G\<close>]:
       "\<^bold>s\<^bold>u\<^bold>b\<^bold>t\<^bold>y\<^bold>p\<^bold>e H \<longmapsto> \<blangle> H \<brangle>  \<^bold>@\<^bold>G\<^bold>O\<^bold>A\<^bold>L G"
@@ -2053,18 +2114,6 @@ lemma [\<phi>reason 4000 on \<open>\<^bold>s\<^bold>u\<^bold>b\<^bold>t\<^bold>y
   for H :: \<open>'a::monoid_mult set\<close>
   unfolding cast_def mult_1_left by blast+
 
-(* lemma [\<phi>intro 40]: \<comment> \<open>outro\<close>
-    "\<^bold>s\<^bold>i\<^bold>m\<^bold>p\<^bold>r\<^bold>e\<^bold>m a = a' \<Longrightarrow>
-    \<^bold>s\<^bold>u\<^bold>b\<^bold>t\<^bold>y\<^bold>p\<^bold>e a \<Zinj> h \<Ztypecolon> H \<longmapsto> H' * a' \<Zinj> x \<Ztypecolon> X \<^bold>w\<^bold>i\<^bold>t\<^bold>h P \<^bold>d\<^bold>u\<^bold>a\<^bold>l H'\<^sub>m * a' \<Zinj> x\<^sub>m \<Ztypecolon> X\<^sub>m \<longmapsto> a \<Zinj> h\<^sub>m \<Ztypecolon> H\<^sub>m \<Longrightarrow>
-      \<^bold>s\<^bold>u\<^bold>b\<^bold>t\<^bold>y\<^bold>p\<^bold>e a \<Zinj> h \<Ztypecolon> H \<longmapsto> H' * \<blangle> Ele \<tort_lbrace> a' \<Zinj> x \<Ztypecolon> X \<tort_rbrace> \<brangle> \<^bold>w\<^bold>i\<^bold>t\<^bold>h P \<^bold>d\<^bold>u\<^bold>a\<^bold>l H'\<^sub>m * \<blangle> a' \<Zinj> x\<^sub>m \<Ztypecolon> X\<^sub>m \<brangle> \<longmapsto> a \<Zinj> h\<^sub>m \<Ztypecolon> H\<^sub>m \<brangle>"
-  and [\<phi>intro 40]:
-    "\<^bold>s\<^bold>i\<^bold>m\<^bold>p\<^bold>r\<^bold>e\<^bold>m a = a' \<Longrightarrow> 
-    \<^bold>s\<^bold>u\<^bold>b\<^bold>t\<^bold>y\<^bold>p\<^bold>e a \<Zinj> h \<Ztypecolon> H \<longmapsto> H' * a' \<Zinj> x \<Ztypecolon> X \<^bold>w\<^bold>i\<^bold>t\<^bold>h P \<Longrightarrow> \<^bold>s\<^bold>u\<^bold>b\<^bold>t\<^bold>y\<^bold>p\<^bold>e a \<Zinj> h \<Ztypecolon> H \<longmapsto> H' * \<blangle> a' \<Zinj> x \<Ztypecolon> X \<brangle> \<^bold>w\<^bold>i\<^bold>t\<^bold>h P \<brangle>"
-  and [\<phi>intro 70]:
-    "\<^bold>s\<^bold>i\<^bold>m\<^bold>p\<^bold>r\<^bold>e\<^bold>m a = a' \<Longrightarrow> \<^bold>s\<^bold>u\<^bold>b\<^bold>t\<^bold>y\<^bold>p\<^bold>e a \<Zinj> h \<Ztypecolon> H \<longmapsto> a' \<Zinj> x \<Ztypecolon> X \<^bold>w\<^bold>i\<^bold>t\<^bold>h P \<Longrightarrow> \<^bold>s\<^bold>u\<^bold>b\<^bold>t\<^bold>y\<^bold>p\<^bold>e a \<Zinj> h \<Ztypecolon> H \<longmapsto> 1 * \<blangle> a' \<Zinj> x \<Ztypecolon> X \<brangle> \<^bold>w\<^bold>i\<^bold>t\<^bold>h P \<brangle>"*)
-(*  and [\<phi>intro 70]:
-    "\<^bold>s\<^bold>u\<^bold>b\<^bold>t\<^bold>y\<^bold>p\<^bold>e h \<Ztypecolon> H \<longmapsto> x \<Ztypecolon> X \<^bold>w\<^bold>i\<^bold>t\<^bold>h P \<Longrightarrow> \<^bold>s\<^bold>u\<^bold>b\<^bold>t\<^bold>y\<^bold>p\<^bold>e h \<Ztypecolon> H \<longmapsto> \<blangle> x \<Ztypecolon> X \<brangle> \<^bold>w\<^bold>i\<^bold>t\<^bold>h P \<brangle>" 
-  unfolding Heap_Subty_Goal_def Separation_emptyL .*)
 
 context std begin
 
@@ -2075,9 +2124,7 @@ lemma [\<phi>reason 2000 ]:
    \<^bold>s\<^bold>u\<^bold>b\<^bold>t\<^bold>y\<^bold>p\<^bold>e H \<longmapsto> \<blangle> X \<heavy_comma> 1 \<brangle> \<^bold>w\<^bold>i\<^bold>t\<^bold>h P \<^bold>@\<^bold>G\<^bold>O\<^bold>A\<^bold>L G"
   unfolding cast_def mult_1_right .
 
-lemma [\<phi>reason 2000
-    if no \<open>\<^bold>s\<^bold>u\<^bold>b\<^bold>t\<^bold>y\<^bold>p\<^bold>e Void \<heavy_comma> Void \<longmapsto> ?X \<^bold>w\<^bold>i\<^bold>t\<^bold>h ?P \<^bold>@\<^bold>G\<^bold>O\<^bold>A\<^bold>L ?G\<close>
-]:
+lemma [\<phi>reason 2000]:
   "\<^bold>s\<^bold>u\<^bold>b\<^bold>t\<^bold>y\<^bold>p\<^bold>e R \<longmapsto> X \<^bold>w\<^bold>i\<^bold>t\<^bold>h P \<^bold>@\<^bold>G\<^bold>O\<^bold>A\<^bold>L G \<Longrightarrow>
    \<^bold>s\<^bold>u\<^bold>b\<^bold>t\<^bold>y\<^bold>p\<^bold>e R \<heavy_comma> Void \<longmapsto> X \<^bold>w\<^bold>i\<^bold>t\<^bold>h P \<^bold>@\<^bold>G\<^bold>O\<^bold>A\<^bold>L G"
   unfolding cast_def mult_1_right .
@@ -2104,26 +2151,21 @@ lemma [\<phi>reason 2000
    \<^bold>s\<^bold>u\<^bold>b\<^bold>t\<^bold>y\<^bold>p\<^bold>e Y \<longmapsto> X \<^bold>w\<^bold>i\<^bold>t\<^bold>h P \<^bold>@\<^bold>G\<^bold>O\<^bold>A\<^bold>L G"
   unfolding cast_def mult_1_left .
 
-lemma [\<phi>reason 2000]:
-  "\<^bold>s\<^bold>u\<^bold>b\<^bold>t\<^bold>y\<^bold>p\<^bold>e 1 \<longmapsto> X \<^bold>w\<^bold>i\<^bold>t\<^bold>h P \<^bold>@\<^bold>G\<^bold>O\<^bold>A\<^bold>L G \<Longrightarrow>
-   \<^bold>s\<^bold>u\<^bold>b\<^bold>t\<^bold>y\<^bold>p\<^bold>e 1\<heavy_comma> 1 \<longmapsto> X \<^bold>w\<^bold>i\<^bold>t\<^bold>h P \<^bold>@\<^bold>G\<^bold>O\<^bold>A\<^bold>L G"
-  unfolding cast_def mult_1_left .
-
 subsubsection \<open>Subjection\<close>
 
-lemma [\<phi>reason 2000]:
+lemma [\<phi>reason 2100]:
   "\<^bold>s\<^bold>u\<^bold>b\<^bold>t\<^bold>y\<^bold>p\<^bold>e T \<longmapsto> \<blangle> U \<brangle> \<^bold>w\<^bold>i\<^bold>t\<^bold>h P \<^bold>@\<^bold>G\<^bold>O\<^bold>A\<^bold>L G \<Longrightarrow>
    (P \<Longrightarrow> \<^bold>p\<^bold>r\<^bold>e\<^bold>m\<^bold>i\<^bold>s\<^bold>e Q) \<Longrightarrow>
    \<^bold>s\<^bold>u\<^bold>b\<^bold>t\<^bold>y\<^bold>p\<^bold>e T \<longmapsto> \<blangle> U \<^bold>s\<^bold>u\<^bold>b\<^bold>j Q \<brangle> \<^bold>w\<^bold>i\<^bold>t\<^bold>h P \<^bold>@\<^bold>G\<^bold>O\<^bold>A\<^bold>L G"
   unfolding cast_def by (simp add: \<phi>expns)
 
-lemma [\<phi>reason 2000]:
-  "\<^bold>s\<^bold>u\<^bold>b\<^bold>t\<^bold>y\<^bold>p\<^bold>e T \<longmapsto> \<blangle> R * U \<brangle> \<^bold>w\<^bold>i\<^bold>t\<^bold>h P \<^bold>@\<^bold>G\<^bold>O\<^bold>A\<^bold>L G \<Longrightarrow>
+lemma [\<phi>reason 2100]:
+  "\<^bold>s\<^bold>u\<^bold>b\<^bold>t\<^bold>y\<^bold>p\<^bold>e T \<longmapsto> \<blangle> R \<heavy_comma> U \<brangle> \<^bold>w\<^bold>i\<^bold>t\<^bold>h P \<^bold>@\<^bold>G\<^bold>O\<^bold>A\<^bold>L G \<Longrightarrow>
    (P \<Longrightarrow> \<^bold>p\<^bold>r\<^bold>e\<^bold>m\<^bold>i\<^bold>s\<^bold>e Q) \<Longrightarrow>
-   \<^bold>s\<^bold>u\<^bold>b\<^bold>t\<^bold>y\<^bold>p\<^bold>e T \<longmapsto> \<blangle> R * (U \<^bold>s\<^bold>u\<^bold>b\<^bold>j Q) \<brangle> \<^bold>w\<^bold>i\<^bold>t\<^bold>h P \<^bold>@\<^bold>G\<^bold>O\<^bold>A\<^bold>L G"
+   \<^bold>s\<^bold>u\<^bold>b\<^bold>t\<^bold>y\<^bold>p\<^bold>e T \<longmapsto> \<blangle> R \<heavy_comma> (U \<^bold>s\<^bold>u\<^bold>b\<^bold>j Q) \<brangle> \<^bold>w\<^bold>i\<^bold>t\<^bold>h P \<^bold>@\<^bold>G\<^bold>O\<^bold>A\<^bold>L G"
   unfolding cast_def by (simp add: \<phi>expns)
 
-lemma [\<phi>reason 2500]:
+lemma [\<phi>reason 2100]:
   "(Q \<Longrightarrow> \<^bold>s\<^bold>u\<^bold>b\<^bold>t\<^bold>y\<^bold>p\<^bold>e T \<longmapsto> U \<^bold>w\<^bold>i\<^bold>t\<^bold>h P \<^bold>@\<^bold>G\<^bold>O\<^bold>A\<^bold>L G) \<Longrightarrow>
    \<^bold>s\<^bold>u\<^bold>b\<^bold>t\<^bold>y\<^bold>p\<^bold>e T \<^bold>s\<^bold>u\<^bold>b\<^bold>j Q \<longmapsto> U \<^bold>w\<^bold>i\<^bold>t\<^bold>h P \<^bold>@\<^bold>G\<^bold>O\<^bold>A\<^bold>L G"
   unfolding cast_def by (simp add: \<phi>expns) blast
@@ -2131,12 +2173,12 @@ lemma [\<phi>reason 2500]:
 
 subsubsection \<open>Existential\<close>
 
-lemma [\<phi>reason 2000]:
+lemma [\<phi>reason 2100]:
   "\<^bold>s\<^bold>u\<^bold>b\<^bold>t\<^bold>y\<^bold>p\<^bold>e T \<longmapsto> \<blangle> U c \<brangle> \<^bold>w\<^bold>i\<^bold>t\<^bold>h P \<^bold>@\<^bold>G\<^bold>O\<^bold>A\<^bold>L G \<Longrightarrow>
    \<^bold>s\<^bold>u\<^bold>b\<^bold>t\<^bold>y\<^bold>p\<^bold>e T \<longmapsto> \<blangle> ExSet U \<brangle> \<^bold>w\<^bold>i\<^bold>t\<^bold>h P \<^bold>@\<^bold>G\<^bold>O\<^bold>A\<^bold>L G"
   unfolding cast_def by (simp add: \<phi>expns) blast
 
-lemma [\<phi>reason 2500]:
+lemma [\<phi>reason 2100]:
   "(\<And>x. \<^bold>s\<^bold>u\<^bold>b\<^bold>t\<^bold>y\<^bold>p\<^bold>e T x \<longmapsto> U \<^bold>w\<^bold>i\<^bold>t\<^bold>h P \<^bold>@\<^bold>G\<^bold>O\<^bold>A\<^bold>L G) \<Longrightarrow>
    \<^bold>s\<^bold>u\<^bold>b\<^bold>t\<^bold>y\<^bold>p\<^bold>e ExSet T \<longmapsto> U \<^bold>w\<^bold>i\<^bold>t\<^bold>h P \<^bold>@\<^bold>G\<^bold>O\<^bold>A\<^bold>L G"
   unfolding cast_def by (simp add: \<phi>expns) blast
@@ -2185,7 +2227,7 @@ lemma [\<phi>reason 3000]:
 \<Longrightarrow> \<^bold>s\<^bold>u\<^bold>b\<^bold>t\<^bold>y\<^bold>p\<^bold>e 0 + Y \<longmapsto> X \<^bold>w\<^bold>i\<^bold>t\<^bold>h P \<^bold>@\<^bold>G\<^bold>O\<^bold>A\<^bold>L G\<close>
   unfolding cast_def by simp
 
-subsubsection \<open>Branch\<close>
+subsubsection \<open>Divergence of Union\<close>
 
 paragraph \<open>Divide Schematic Variable\<close>
 
@@ -2237,7 +2279,7 @@ lemma (in std) [\<phi>reason 1200 on \<open>PROP ALSTR_Divide_Assertion_U \<blan
 
 paragraph \<open>Main Rules\<close>
 
-lemma [\<phi>reason 2500 on \<open>\<^bold>s\<^bold>u\<^bold>b\<^bold>t\<^bold>y\<^bold>p\<^bold>e ?A + ?B \<longmapsto> ?X \<^bold>w\<^bold>i\<^bold>t\<^bold>h ?P \<^bold>@\<^bold>G\<^bold>O\<^bold>A\<^bold>L ?G\<close>]:
+lemma [\<phi>reason 2000 on \<open>\<^bold>s\<^bold>u\<^bold>b\<^bold>t\<^bold>y\<^bold>p\<^bold>e ?A + ?B \<longmapsto> ?X \<^bold>w\<^bold>i\<^bold>t\<^bold>h ?P \<^bold>@\<^bold>G\<^bold>O\<^bold>A\<^bold>L ?G\<close>]:
   \<open> PROP ALSTR_Divide_Assertion_U X XA XB
 \<Longrightarrow> SUBGOAL G G1
 \<Longrightarrow> \<^bold>s\<^bold>u\<^bold>b\<^bold>t\<^bold>y\<^bold>p\<^bold>e B \<longmapsto> XB \<^bold>w\<^bold>i\<^bold>t\<^bold>h P1 \<^bold>@\<^bold>G\<^bold>O\<^bold>A\<^bold>L G1
@@ -2246,7 +2288,7 @@ lemma [\<phi>reason 2500 on \<open>\<^bold>s\<^bold>u\<^bold>b\<^bold>t\<^bold>y
 \<Longrightarrow> \<^bold>s\<^bold>u\<^bold>b\<^bold>t\<^bold>y\<^bold>p\<^bold>e A + B \<longmapsto> X \<^bold>w\<^bold>i\<^bold>t\<^bold>h P1 \<or> P2 \<^bold>@\<^bold>G\<^bold>O\<^bold>A\<^bold>L G\<close>
   unfolding cast_def plus_set_def ALSTR_Divide_Assertion_U_def by simp
 
-lemma [\<phi>reason 2500 on \<open>\<^bold>s\<^bold>u\<^bold>b\<^bold>t\<^bold>y\<^bold>p\<^bold>e ?R\<heavy_comma> (?A + ?B) \<longmapsto> ?X \<^bold>w\<^bold>i\<^bold>t\<^bold>h ?P \<^bold>@\<^bold>G\<^bold>O\<^bold>A\<^bold>L ?G\<close>]:
+lemma [\<phi>reason 2000 on \<open>\<^bold>s\<^bold>u\<^bold>b\<^bold>t\<^bold>y\<^bold>p\<^bold>e ?R\<heavy_comma> (?A + ?B) \<longmapsto> ?X \<^bold>w\<^bold>i\<^bold>t\<^bold>h ?P \<^bold>@\<^bold>G\<^bold>O\<^bold>A\<^bold>L ?G\<close>]:
   \<open> PROP ALSTR_Divide_Assertion_U X XA XB
 \<Longrightarrow> SUBGOAL G G1
 \<Longrightarrow> \<^bold>s\<^bold>u\<^bold>b\<^bold>t\<^bold>y\<^bold>p\<^bold>e R\<heavy_comma> B \<longmapsto> XB \<^bold>w\<^bold>i\<^bold>t\<^bold>h P1 \<^bold>@\<^bold>G\<^bold>O\<^bold>A\<^bold>L G1
@@ -2275,12 +2317,15 @@ lemma [\<phi>reason 800]:
 \<Longrightarrow> \<^bold>s\<^bold>u\<^bold>b\<^bold>t\<^bold>y\<^bold>p\<^bold>e X \<longmapsto> R\<heavy_comma> \<blangle> A + B \<brangle> \<^bold>w\<^bold>i\<^bold>t\<^bold>h P \<^bold>@\<^bold>G\<^bold>O\<^bold>A\<^bold>L G\<close>
   unfolding cast_def by (simp add: distrib_left)
 
-subsubsection \<open>General\<close>
+subsubsection \<open>Step-by-Step Searching Procedure\<close>
 
-lemma [\<phi>reason 2000 on \<open>\<^bold>s\<^bold>u\<^bold>b\<^bold>t\<^bold>y\<^bold>p\<^bold>e ?R \<longmapsto> \<blangle> ?R2 \<heavy_comma> ?X \<brangle> \<^bold>w\<^bold>i\<^bold>t\<^bold>h ?P \<^bold>@\<^bold>G\<^bold>O\<^bold>A\<^bold>L ?G\<close>]:
-  " \<^bold>s\<^bold>u\<^bold>b\<^bold>t\<^bold>y\<^bold>p\<^bold>e R \<longmapsto> R1 \<heavy_comma> \<blangle> X \<brangle> \<^bold>w\<^bold>i\<^bold>t\<^bold>h P1 \<^bold>@\<^bold>G\<^bold>O\<^bold>A\<^bold>L G
-\<Longrightarrow> \<^bold>s\<^bold>u\<^bold>b\<^bold>t\<^bold>y\<^bold>p\<^bold>e R1 \<longmapsto> \<blangle> R2 \<brangle> \<^bold>w\<^bold>i\<^bold>t\<^bold>h P2  \<^bold>@\<^bold>G\<^bold>O\<^bold>A\<^bold>L G
-\<Longrightarrow> \<^bold>s\<^bold>u\<^bold>b\<^bold>t\<^bold>y\<^bold>p\<^bold>e R \<longmapsto> \<blangle> R2 \<heavy_comma> X \<brangle> \<^bold>w\<^bold>i\<^bold>t\<^bold>h P1 \<and> P2 \<^bold>@\<^bold>G\<^bold>O\<^bold>A\<^bold>L G"
+lemma [\<phi>reason 2000
+    on \<open>\<^bold>s\<^bold>u\<^bold>b\<^bold>t\<^bold>y\<^bold>p\<^bold>e ?R \<longmapsto> \<blangle> ?R2 \<heavy_comma> ?X \<brangle> \<^bold>w\<^bold>i\<^bold>t\<^bold>h ?P \<^bold>@\<^bold>G\<^bold>O\<^bold>A\<^bold>L ?G\<close>
+ if no \<open>\<^bold>s\<^bold>u\<^bold>b\<^bold>t\<^bold>y\<^bold>p\<^bold>e ?R \<longmapsto> \<blangle> ?R2 \<heavy_comma> FIX ?X \<brangle> \<^bold>w\<^bold>i\<^bold>t\<^bold>h ?P \<^bold>@\<^bold>G\<^bold>O\<^bold>A\<^bold>L ?G\<close>
+]:
+  " \<^bold>s\<^bold>u\<^bold>b\<^bold>t\<^bold>y\<^bold>p\<^bold>e R  \<longmapsto> R1 \<heavy_comma> \<blangle> X \<brangle> \<^bold>w\<^bold>i\<^bold>t\<^bold>h P1 \<^bold>@\<^bold>G\<^bold>O\<^bold>A\<^bold>L G
+\<Longrightarrow> \<^bold>s\<^bold>u\<^bold>b\<^bold>t\<^bold>y\<^bold>p\<^bold>e R1 \<longmapsto> \<blangle> R2 \<brangle>     \<^bold>w\<^bold>i\<^bold>t\<^bold>h P2 \<^bold>@\<^bold>G\<^bold>O\<^bold>A\<^bold>L G
+\<Longrightarrow> \<^bold>s\<^bold>u\<^bold>b\<^bold>t\<^bold>y\<^bold>p\<^bold>e R  \<longmapsto> \<blangle> R2 \<heavy_comma> X \<brangle> \<^bold>w\<^bold>i\<^bold>t\<^bold>h P1 \<and> P2 \<^bold>@\<^bold>G\<^bold>O\<^bold>A\<^bold>L G"
   unfolding cast_def pair_forall
   by (simp add: \<phi>expns) metis
 
@@ -2297,9 +2342,9 @@ lemma [\<phi>reason 2000 on \<open>\<^bold>s\<^bold>u\<^bold>b\<^bold>t\<^bold>y
   unfolding cast_def pair_forall
   by (simp add: \<phi>expns)
 
-lemma [\<phi>reason 2000 on \<open>\<^bold>s\<^bold>u\<^bold>b\<^bold>t\<^bold>y\<^bold>p\<^bold>e ?R \<longmapsto> \<blangle> ?R2 \<heavy_comma> SYNTHESIS ?X \<brangle> \<^bold>w\<^bold>i\<^bold>t\<^bold>h ?P \<^bold>@\<^bold>G\<^bold>O\<^bold>A\<^bold>L ?G\<close>]:
-  " \<^bold>s\<^bold>u\<^bold>b\<^bold>t\<^bold>y\<^bold>p\<^bold>e R \<longmapsto> \<blangle> R2 \<heavy_comma> X \<brangle> \<^bold>w\<^bold>i\<^bold>t\<^bold>h P \<^bold>@\<^bold>G\<^bold>O\<^bold>A\<^bold>L G
-\<Longrightarrow> \<^bold>s\<^bold>u\<^bold>b\<^bold>t\<^bold>y\<^bold>p\<^bold>e R \<longmapsto> \<blangle> R2 \<heavy_comma> SYNTHESIS X \<brangle> \<^bold>w\<^bold>i\<^bold>t\<^bold>h P \<^bold>@\<^bold>G\<^bold>O\<^bold>A\<^bold>L G"
+lemma [\<phi>reason 2000 on \<open>\<^bold>s\<^bold>u\<^bold>b\<^bold>t\<^bold>y\<^bold>p\<^bold>e ?R \<longmapsto> ?R2 \<heavy_comma> \<blangle> SYNTHESIS ?X \<brangle> \<^bold>w\<^bold>i\<^bold>t\<^bold>h ?P \<^bold>@\<^bold>G\<^bold>O\<^bold>A\<^bold>L ?G\<close>]:
+  " \<^bold>s\<^bold>u\<^bold>b\<^bold>t\<^bold>y\<^bold>p\<^bold>e R \<longmapsto> R2 \<heavy_comma> \<blangle> X \<brangle> \<^bold>w\<^bold>i\<^bold>t\<^bold>h P \<^bold>@\<^bold>G\<^bold>O\<^bold>A\<^bold>L G
+\<Longrightarrow> \<^bold>s\<^bold>u\<^bold>b\<^bold>t\<^bold>y\<^bold>p\<^bold>e R \<longmapsto> R2 \<heavy_comma> \<blangle> SYNTHESIS X \<brangle> \<^bold>w\<^bold>i\<^bold>t\<^bold>h P \<^bold>@\<^bold>G\<^bold>O\<^bold>A\<^bold>L G"
   unfolding Synthesis_def .
 
 lemma [\<phi>reason 2000 on \<open>\<^bold>s\<^bold>u\<^bold>b\<^bold>t\<^bold>y\<^bold>p\<^bold>e ?R\<heavy_comma> SYNTHESIS ?Y \<longmapsto> ?X \<^bold>w\<^bold>i\<^bold>t\<^bold>h ?P \<^bold>@\<^bold>G\<^bold>O\<^bold>A\<^bold>L ?G\<close>]:
@@ -2308,8 +2353,9 @@ lemma [\<phi>reason 2000 on \<open>\<^bold>s\<^bold>u\<^bold>b\<^bold>t\<^bold>y
   unfolding cast_def pair_forall
   by (simp add: \<phi>expns)
 
-lemma [\<phi>reason 2500 on \<open>\<^bold>s\<^bold>u\<^bold>b\<^bold>t\<^bold>y\<^bold>p\<^bold>e ?R \<heavy_comma> ?V \<longmapsto> ?R' \<heavy_comma> \<blangle> ?X \<brangle> \<^bold>w\<^bold>i\<^bold>t\<^bold>h ?P \<^bold>@\<^bold>G\<^bold>O\<^bold>A\<^bold>L ?G\<close>]:
+lemma [\<phi>reason 2300 on \<open>\<^bold>s\<^bold>u\<^bold>b\<^bold>t\<^bold>y\<^bold>p\<^bold>e ?R \<heavy_comma> ?V \<longmapsto> ?R' \<heavy_comma> \<blangle> ?X \<brangle> \<^bold>w\<^bold>i\<^bold>t\<^bold>h ?P \<^bold>@\<^bold>G\<^bold>O\<^bold>A\<^bold>L ?G\<close>]:
   "\<^bold>s\<^bold>u\<^bold>b\<^bold>t\<^bold>y\<^bold>p\<^bold>e R \<heavy_comma> X \<longmapsto> R \<heavy_comma> \<blangle> X \<brangle> \<^bold>@\<^bold>G\<^bold>O\<^bold>A\<^bold>L G"
+      \<comment> \<open>successful termination of the step-by-step search\<close>
   unfolding cast_def pair_forall
   by (simp add: \<phi>expns times_list_def)
 
@@ -2317,6 +2363,7 @@ lemma [\<phi>reason 2500 on \<open>\<^bold>s\<^bold>u\<^bold>b\<^bold>t\<^bold>y
 subsubsection \<open>Value\<close>
 
 text \<open>The rules require the same values are alpha-conversible. \<close>
+text \<open>Priority shouldn't exceed 2000.\<close>
 
 lemma [\<phi>reason 1500 on \<open>\<^bold>s\<^bold>u\<^bold>b\<^bold>t\<^bold>y\<^bold>p\<^bold>e ?R\<heavy_comma> ?y \<Ztypecolon> Val ?v ?U \<longmapsto> ?R''' \<heavy_comma> \<blangle> ?x \<Ztypecolon> Val ?v' ?T \<brangle> \<^bold>w\<^bold>i\<^bold>t\<^bold>h ?P \<^bold>@\<^bold>G\<^bold>O\<^bold>A\<^bold>L ?G\<close>]:
   " \<^bold>s\<^bold>u\<^bold>b\<^bold>t\<^bold>y\<^bold>p\<^bold>e y \<Ztypecolon> U \<longmapsto> x \<Ztypecolon> T \<^bold>w\<^bold>i\<^bold>t\<^bold>h P
@@ -2390,84 +2437,6 @@ lemma [\<phi>reason 2000]:
   unfolding mult.assoc[symmetric] .
 
 end
-
-(*
-subsection \<open>Scan\<close>
-
-lemma [\<phi>intro 110]:
-  "\<^bold>s\<^bold>u\<^bold>b\<^bold>t\<^bold>y\<^bold>p\<^bold>e R \<longmapsto> R' * \<blangle> VAL X \<brangle> \<^bold>w\<^bold>i\<^bold>t\<^bold>h P \<brangle>
-  \<Longrightarrow> \<^bold>s\<^bold>u\<^bold>b\<^bold>t\<^bold>y\<^bold>p\<^bold>e L * R \<longmapsto> L * R' * \<blangle> VAL X \<brangle> \<^bold>w\<^bold>i\<^bold>t\<^bold>h P \<brangle>"
-  unfolding cast_def Intro_def Dest_def pair_forall
-  by (metis Separation_assoc Separation_expn)
-
-lemma [\<phi>intro 110]:
-  "\<^bold>s\<^bold>u\<^bold>b\<^bold>t\<^bold>y\<^bold>p\<^bold>e R \<longmapsto> R' * \<blangle> OBJ X \<brangle> \<^bold>w\<^bold>i\<^bold>t\<^bold>h P \<brangle>
-  \<Longrightarrow> \<^bold>s\<^bold>u\<^bold>b\<^bold>t\<^bold>y\<^bold>p\<^bold>e L * R \<longmapsto> L * R' * \<blangle> OBJ X \<brangle> \<^bold>w\<^bold>i\<^bold>t\<^bold>h P \<brangle>"
-  unfolding cast_def Intro_def Dest_def pair_forall
-  by (metis Separation_assoc Separation_expn)
-
-lemma [\<phi>intro 100]:
-  "\<^bold>s\<^bold>u\<^bold>b\<^bold>t\<^bold>y\<^bold>p\<^bold>e L \<longmapsto> L' * \<blangle> x \<Ztypecolon> X \<brangle> \<^bold>w\<^bold>i\<^bold>t\<^bold>h P \<brangle>
-  \<Longrightarrow> \<^bold>s\<^bold>u\<^bold>b\<^bold>t\<^bold>y\<^bold>p\<^bold>e H * R \<longmapsto> H' * R * \<blangle> x \<Ztypecolon> X \<brangle> \<^bold>w\<^bold>i\<^bold>t\<^bold>h P \<brangle>"
-  unfolding Subty_def SubtyDual_def Heap_Subty_Goal_def Intro_def Dest_def
-    Separation_comm[of H R] Separation_comm[of H' R]
-  by (metis Heap_Divider_exps Separation_assoc)
-
- 
-
-
-
-
-
-
-lemma heap_idx_R_dual[\<phi>intro 100]:
-  "\<^bold>s\<^bold>u\<^bold>b\<^bold>t\<^bold>y\<^bold>p\<^bold>e H \<longmapsto> H' * \<blangle> x \<Ztypecolon> X \<brangle> \<^bold>w\<^bold>i\<^bold>t\<^bold>h P \<^bold>d\<^bold>u\<^bold>a\<^bold>l H'\<^sub>m * \<blangle> x\<^sub>m \<Ztypecolon> X\<^sub>m \<brangle> \<longmapsto> H\<^sub>m \<brangle>
-  \<Longrightarrow> \<^bold>s\<^bold>u\<^bold>b\<^bold>t\<^bold>y\<^bold>p\<^bold>e H * R \<longmapsto> H' * R * \<blangle> x \<Ztypecolon> X \<brangle> \<^bold>w\<^bold>i\<^bold>t\<^bold>h P \<^bold>d\<^bold>u\<^bold>a\<^bold>l H'\<^sub>m * R * \<blangle> x\<^sub>m \<Ztypecolon> X\<^sub>m \<brangle> \<longmapsto> H\<^sub>m * R \<brangle>"
-  unfolding Subty_def SubtyDual_def Heap_Subty_Goal_def Intro_def Dest_def
-    Separation_comm[of H R] Separation_comm[of H\<^sub>m R]
-    Separation_comm[of H' R] Separation_comm[of H'\<^sub>m R]
-  by (metis Heap_Divider_exps Separation_assoc)
-
-
-
-
-lemma [\<phi>intro 120]:
-  "\<^bold>s\<^bold>u\<^bold>b\<^bold>t\<^bold>y\<^bold>p\<^bold>e H \<longmapsto> H1 * x \<Ztypecolon> \<blangle> X \<brangle> \<^bold>w\<^bold>i\<^bold>t\<^bold>h P1 \<brangle>
-    \<Longrightarrow> (P1 \<Longrightarrow> \<^bold>s\<^bold>u\<^bold>b\<^bold>t\<^bold>y\<^bold>p\<^bold>e H1 \<longmapsto> H\<^sub>r * h2 \<Ztypecolon> \<blangle> H2 \<brangle> \<^bold>w\<^bold>i\<^bold>t\<^bold>h P2 \<brangle>)
-    \<Longrightarrow> \<^bold>s\<^bold>u\<^bold>b\<^bold>t\<^bold>y\<^bold>p\<^bold>e H \<longmapsto> H\<^sub>r * (x, h2) \<Ztypecolon> \<blangle> X \<^emph> H2 \<brangle> \<^bold>w\<^bold>i\<^bold>t\<^bold>h P1 \<and> P2 \<brangle>"
-  unfolding Subty_def SubtyDual_def Heap_Subty_Goal_def HeapDivNu_to_SepSet SepNu_to_SepSet Intro_def Dest_def
-  by (smt (verit, del_insts) SeparationSet_assoc SeparationSet_comm SeparationSet_def mem_Collect_eq)
-*)
-(* lemma [ \<phi>intro -50 ]: "\<^bold>d\<^bold>e\<^bold>s\<^bold>t \<^bold>s\<^bold>u\<^bold>b\<^bold>t\<^bold>y\<^bold>p\<^bold>e x \<Ztypecolon> T \<longmapsto> d \<Ztypecolon> D \<^bold>w\<^bold>i\<^bold>t\<^bold>h P
-  \<Longrightarrow> (P \<Longrightarrow> \<^bold>s\<^bold>u\<^bold>b\<^bold>t\<^bold>y\<^bold>p\<^bold>e d \<Ztypecolon> D \<longmapsto> d' \<Ztypecolon> D' * h \<Ztypecolon> \<blangle> H \<brangle> \<^bold>w\<^bold>i\<^bold>t\<^bold>h P2 \<^bold>d\<^bold>u\<^bold>a\<^bold>l i'\<^sub>m \<Ztypecolon> I'\<^sub>m * h\<^sub>m \<Ztypecolon> \<blangle> H\<^sub>m \<brangle> \<longmapsto> i \<Ztypecolon> I \<brangle>)
-  \<Longrightarrow> (P \<Longrightarrow> P2 \<Longrightarrow> \<^bold>i\<^bold>n\<^bold>t\<^bold>r\<^bold>o \<^bold>s\<^bold>u\<^bold>b\<^bold>t\<^bold>y\<^bold>p\<^bold>e i \<Ztypecolon> I \<longmapsto> x\<^sub>m \<Ztypecolon> T \<^bold>w\<^bold>i\<^bold>t\<^bold>h Anyway)
-  \<Longrightarrow> \<^bold>s\<^bold>u\<^bold>b\<^bold>t\<^bold>y\<^bold>p\<^bold>e x \<Ztypecolon> T \<longmapsto> d' \<Ztypecolon> D' * h \<Ztypecolon> \<blangle> H \<brangle> \<^bold>w\<^bold>i\<^bold>t\<^bold>h P \<and> P2 \<^bold>d\<^bold>u\<^bold>a\<^bold>l i'\<^sub>m \<Ztypecolon> I'\<^sub>m * h\<^sub>m \<Ztypecolon> \<blangle> H\<^sub>m \<brangle> \<longmapsto> x\<^sub>m \<Ztypecolon> T \<brangle>"
-  unfolding Dest_def Intro_def SubtyDual_def Different_def Heap_Subty_Goal_def Subty_def
-  by (auto simp add: Premise_def) *)
-
-(* lemma [ \<phi>intro 50 ]: "\<^bold>s\<^bold>u\<^bold>b\<^bold>t\<^bold>y\<^bold>p\<^bold>e x \<Ztypecolon> T \<longmapsto> d \<Ztypecolon> D \<^bold>w\<^bold>i\<^bold>t\<^bold>h P
-  \<Longrightarrow> (P \<Longrightarrow> \<^bold>s\<^bold>u\<^bold>b\<^bold>t\<^bold>y\<^bold>p\<^bold>e d \<Ztypecolon> D \<longmapsto> d' \<Ztypecolon> D' * h \<Ztypecolon> \<blangle> H \<brangle> \<^bold>w\<^bold>i\<^bold>t\<^bold>h P2 \<^bold>d\<^bold>u\<^bold>a\<^bold>l i'\<^sub>m \<Ztypecolon> I'\<^sub>m * h\<^sub>m \<Ztypecolon> \<blangle> H\<^sub>m \<brangle> \<longmapsto> i \<Ztypecolon> I \<brangle>)
-  \<Longrightarrow> (P \<Longrightarrow> P2 \<Longrightarrow> \<^bold>i\<^bold>n\<^bold>t\<^bold>r\<^bold>o \<^bold>s\<^bold>u\<^bold>b\<^bold>t\<^bold>y\<^bold>p\<^bold>e i \<Ztypecolon> I \<longmapsto> x\<^sub>m \<Ztypecolon> T \<^bold>w\<^bold>i\<^bold>t\<^bold>h Anyway)
-  \<Longrightarrow> \<^bold>s\<^bold>u\<^bold>b\<^bold>t\<^bold>y\<^bold>p\<^bold>e x \<Ztypecolon> T \<longmapsto> d' \<Ztypecolon> D' * h \<Ztypecolon> \<blangle> H \<brangle> \<^bold>w\<^bold>i\<^bold>t\<^bold>h P \<and> P2 \<brangle>"
-  unfolding Dest_def Intro_def SubtyDual_def Different_def Heap_Subty_Goal_def Subty_def
-  by (auto simp add: Premise_def) *)
-
-
-
-(* lemma heap_put_this: "\<^bold>s\<^bold>u\<^bold>b\<^bold>t\<^bold>y\<^bold>p\<^bold>e 1 * x \<Ztypecolon> X \<longmapsto> x \<Ztypecolon> X" unfolding Subty_def Separation_emptyL by simp
-lemma "\<^bold>s\<^bold>u\<^bold>b\<^bold>t\<^bold>y\<^bold>p\<^bold>e s \<Ztypecolon> S * x \<Ztypecolon> X \<longmapsto> s' \<Ztypecolon> S' \<Longrightarrow> \<^bold>s\<^bold>u\<^bold>b\<^bold>t\<^bold>y\<^bold>p\<^bold>e l \<Ztypecolon> L * s \<Ztypecolon> S * x \<Ztypecolon> X \<longmapsto> l \<Ztypecolon> L * s' \<Ztypecolon> S' "
-  unfolding Subty_def HeapDivNu_to_SepSet
-  by (smt (verit, del_insts) SeparationSet_assoc SeparationSet_comm SeparationSet_def mem_Collect_eq)
-lemma "\<^bold>s\<^bold>u\<^bold>b\<^bold>t\<^bold>y\<^bold>p\<^bold>e s \<Ztypecolon> S * x \<Ztypecolon> X \<longmapsto> s' \<Ztypecolon> S' \<Longrightarrow> \<^bold>s\<^bold>u\<^bold>b\<^bold>t\<^bold>y\<^bold>p\<^bold>e (s \<Ztypecolon> S * r \<Ztypecolon> R) * x \<Ztypecolon> X \<longmapsto> s' \<Ztypecolon> S' * r \<Ztypecolon> R "
-  unfolding Subty_def HeapDivNu_to_SepSet
-  by (smt (verit, del_insts) SeparationSet_assoc SeparationSet_comm SeparationSet_def mem_Collect_eq)
-*)
-
-
-(* lemma "\<^bold>s\<^bold>u\<^bold>b\<^bold>t\<^bold>y\<^bold>p\<^bold>e S \<longmapsto> S' \<Longrightarrow> \<^bold>s\<^bold>u\<^bold>b\<^bold>t\<^bold>y\<^bold>p\<^bold>e L * S \<longmapsto> L * S'"
-  unfolding Subty_def by (smt (verit, del_insts) Separation_assoc Separation_comm Separation_def mem_Collect_eq
-lemma "\<^bold>s\<^bold>u\<^bold>b\<^bold>t\<^bold>y\<^bold>p\<^bold>e S \<longmapsto> S' \<Longrightarrow> \<^bold>s\<^bold>u\<^bold>b\<^bold>t\<^bold>y\<^bold>p\<^bold>e S * R \<longmapsto> S' * R"
-  unfolding Subty_def by (smt (verit, del_insts) Separation_assoc Separation_comm Separation_def mem_Collect_eq *)
 
 
 (*
@@ -2716,6 +2685,71 @@ lemma Prog_Interface_func:
   "TERM f \<Longrightarrow> Prog_Interface name TYPE('a::lrep) TYPE('b::lrep) f" 
   unfolding Prog_Interface_def ..
 *)
+
+subsection \<open>Filter Out Values\<close>
+
+definition \<open>Filter_Out_Values'' \<equiv> Filter_Out_Values\<close>
+definition \<open>Filter_Out_Values' (remain::'a::times set) (keep::'a set) (check::'a set) (ret::'a set)
+              \<equiv> Trueprop (keep = check \<longrightarrow> (\<^bold>s\<^bold>u\<^bold>b\<^bold>t\<^bold>y\<^bold>p\<^bold>e remain * keep \<longmapsto> ret))\<close>
+
+lemma [\<phi>reason on \<open>PROP Filter_Out_Values ?X ?Z\<close>]:
+  \<open> Simplify assertion_simplification X' X
+\<Longrightarrow> PROP Filter_Out_Values'' X' Z
+\<Longrightarrow> PROP Filter_Out_Values X Z\<close>
+  unfolding Filter_Out_Values''_def Simplify_def by simp
+
+lemma [\<phi>reason on \<open>PROP Filter_Out_Values ?var_X ?Z\<close>]:
+  \<open>PROP Filter_Out_Values X X\<close>
+  unfolding Filter_Out_Values_def using cast_id .
+
+lemma [\<phi>reason 1200 on \<open>PROP Filter_Out_Values'' (ExSet ?T) ?T'\<close>]:
+  \<open>(\<And>c. PROP Filter_Out_Values'' (T c) (T' c))
+\<Longrightarrow> PROP Filter_Out_Values'' (ExSet T) (ExSet T')\<close>
+  unfolding Filter_Out_Values_def Filter_Out_Values''_def Subty_def
+  by (simp add: \<phi>expns) blast
+
+lemma [\<phi>reason 1200 on \<open>PROP Filter_Out_Values'' (?T \<^bold>s\<^bold>u\<^bold>b\<^bold>j ?P) ?T'\<close>]:
+  \<open> PROP Filter_Out_Values'' T T'
+\<Longrightarrow> PROP Filter_Out_Values'' (T \<^bold>s\<^bold>u\<^bold>b\<^bold>j P) (T' \<^bold>s\<^bold>u\<^bold>b\<^bold>j P)\<close>
+  unfolding Filter_Out_Values_def Subty_def Filter_Out_Values''_def
+  by (simp add: \<phi>expns)
+
+lemma (in std) [\<phi>reason 1200 on \<open>PROP Filter_Out_Values'' (?R\<heavy_comma> ?X) ?Z\<close>]:
+  \<open> PROP Filter_Out_Values'' R R'
+\<Longrightarrow> PROP Filter_Out_Values' R' X X Z
+\<Longrightarrow> PROP Filter_Out_Values'' (R\<heavy_comma> X) Z\<close>
+  unfolding Filter_Out_Values_def Subty_def Filter_Out_Values'_def Filter_Out_Values''_def
+  by (simp add: \<phi>expns) blast
+
+lemma (in std) [\<phi>reason 1100 on \<open>PROP Filter_Out_Values'' ?R ?Z\<close>]:
+  \<open> PROP Filter_Out_Values' Void R R Z
+\<Longrightarrow> PROP Filter_Out_Values'' R Z\<close>
+  unfolding Filter_Out_Values_def Filter_Out_Values'_def Subty_def Filter_Out_Values''_def
+  by simp
+
+lemma [\<phi>reason 1200 on \<open>PROP Filter_Out_Values' ?R ?Y (SYNTHESIS ?X) ?Z\<close>]:
+  \<open> PROP Filter_Out_Values' R Y X Z
+\<Longrightarrow> PROP Filter_Out_Values' R Y (SYNTHESIS X) Z\<close>
+  unfolding Filter_Out_Values'_def Synthesis_def .
+
+lemma [\<phi>reason 1200 on \<open>PROP Filter_Out_Values' ?R ?Y (FIX ?X) ?Z\<close>]:
+  \<open> PROP Filter_Out_Values' R Y X Z
+\<Longrightarrow> PROP Filter_Out_Values' R Y (FIX X) Z\<close>
+  unfolding Filter_Out_Values'_def Fix_def .
+
+lemma (in std) [\<phi>reason 1200 on \<open>PROP Filter_Out_Values' ?R ?Y (?x \<Ztypecolon> Val ?raw ?T) ?Z\<close>]:
+  \<open>PROP Filter_Out_Values' R Y (x \<Ztypecolon> Val raw T) R\<close>
+  unfolding Filter_Out_Values'_def Subty_def by (simp add: \<phi>expns)
+
+lemma (in std) [\<phi>reason 1100 on \<open>PROP Filter_Out_Values' Void ?Y ?X ?Z\<close>]:
+  \<open>PROP Filter_Out_Values' Void Y X Y\<close>
+  unfolding Filter_Out_Values'_def Subty_def by simp
+
+lemma (in std) [\<phi>reason 1080 on \<open>PROP Filter_Out_Values' ?R ?Y ?X ?Z\<close>]:
+  \<open>PROP Filter_Out_Values' R Y X (R\<heavy_comma> Y)\<close>
+  unfolding Filter_Out_Values'_def Subty_def by simp
+
+
 
 section \<open>Implementation of the Language\<close>
 
