NuStd_Base.thy
@@ -112,10 +112,9 @@ proc op_set_var__synthesis[
   \<phi>reason on \<open>\<^bold>p\<^bold>r\<^bold>o\<^bold>c ?f \<lbrace> ?R \<longmapsto> \<lambda>ret. ?R'\<heavy_comma> SYNTHESIS ($?var := ?y) \<Ztypecolon> ?U ret \<^bold>t\<^bold>h\<^bold>r\<^bold>o\<^bold>w\<^bold>s ?E \<rbrace> \<^bold>@\<^bold>G\<^bold>O\<^bold>A\<^bold>L ?G\<close>
 ]:
 assumes G: \<open>\<^bold>p\<^bold>r\<^bold>o\<^bold>c g \<lbrace> X \<longmapsto> X1\<heavy_comma> SYNTHESIS \<^bold>v\<^bold>a\<^bold>l y \<Ztypecolon> U \<^bold>t\<^bold>h\<^bold>r\<^bold>o\<^bold>w\<^bold>s E\<rbrace> \<^bold>@\<^bold>G\<^bold>O\<^bold>A\<^bold>L G \<close>
-  and      \<open>SUBGOAL G G2\<close>
-  and S[unfolded GOAL_CTXT_def FOCUS_TAG_def]:
-        \<open>\<And>vy. \<^bold>s\<^bold>u\<^bold>b\<^bold>t\<^bold>y\<^bold>p\<^bold>e X1\<heavy_comma> y \<Ztypecolon> Val vy U \<longmapsto> \<blangle> Y\<heavy_comma> x \<Ztypecolon> Var var T\<heavy_comma> y \<Ztypecolon> Val vy U \<brangle> \<^bold>w\<^bold>i\<^bold>t\<^bold>h Any \<^bold>@\<^bold>G\<^bold>O\<^bold>A\<^bold>L G2\<close>
-  and   \<open>SOLVE_SUBGOAL G2\<close>
+  and S[unfolded Assertion_Level_SubType_Reasoning_def]:
+        \<open>\<And>vy. PROP Assertion_Level_SubType_Reasoning(
+                  \<^bold>s\<^bold>u\<^bold>b\<^bold>t\<^bold>y\<^bold>p\<^bold>e X1\<heavy_comma> y \<Ztypecolon> Val vy U \<longmapsto> \<blangle> Y\<heavy_comma> x \<Ztypecolon> Var var T\<heavy_comma> y \<Ztypecolon> Val vy U \<brangle> \<^bold>w\<^bold>i\<^bold>t\<^bold>h Any)\<close>
   and [\<phi>reason on \<open>\<phi>SemType (x \<Ztypecolon> T) ?TY\<close>]: \<open>\<phi>SemType (x \<Ztypecolon> T) TY\<close>
   and [\<phi>reason on \<open>\<phi>SemType (y \<Ztypecolon> U) ?TY\<close>]: \<open>\<phi>SemType (y \<Ztypecolon> U) TY\<close>
  goal G
@@ -136,7 +135,7 @@ proc (in std) op_var_scope:
   return   \<open>Y\<close>
   throws   E
   \<medium_left_bracket> to_Identity op_var_scope';;
-    try'' ;; \<medium_left_bracket> BLK to_Identity op_free_var \<medium_right_bracket>. \<medium_left_bracket> to_Identity op_free_var;; throw \<medium_right_bracket>. \<medium_right_bracket>. .
+    try'' ;; \<medium_left_bracket> BLK to_Identity ;; op_free_var \<medium_right_bracket> .. \<medium_left_bracket> to_Identity op_free_var;; throw \<medium_right_bracket>. \<medium_right_bracket>. .
 
 
 lemma "__\<phi>op_var_scope__":
@@ -187,7 +186,7 @@ lemma (in std) op_not[\<phi>overload \<not>]:
   unfolding op_not_def
   by (cases raw, simp, \<phi>reason)
 
-proc "\<phi>__synthesis_lneg"[
+proc [
     \<phi>reason on \<open>\<^bold>p\<^bold>r\<^bold>o\<^bold>c ?F \<lbrace> ?R \<longmapsto> \<lambda>ret. ?R1\<heavy_comma> SYNTHESIS \<not>?b \<Ztypecolon> ?T ret \<^bold>t\<^bold>h\<^bold>r\<^bold>o\<^bold>w\<^bold>s ?E \<rbrace> \<^bold>@\<^bold>G\<^bold>O\<^bold>A\<^bold>L ?G\<close>
 ]:
   assumes F1: \<open>\<^bold>p\<^bold>r\<^bold>o\<^bold>c f \<lbrace> R \<longmapsto> R1\<heavy_comma> SYNTHESIS \<^bold>v\<^bold>a\<^bold>l b \<Ztypecolon> \<bool> \<rbrace>  \<^bold>@\<^bold>G\<^bold>O\<^bold>A\<^bold>L G\<close>
@@ -204,7 +203,7 @@ lemma (in std) op_and[\<phi>overload \<and>]:
   by (cases va; cases vb; simp, \<phi>reason)
 
 
-proc "\<phi>__synthesis_land"[
+proc [
     \<phi>reason on \<open>\<^bold>p\<^bold>r\<^bold>o\<^bold>c ?F \<lbrace> ?R \<longmapsto> \<lambda>ret. ?R2\<heavy_comma> SYNTHESIS (?x \<and> ?y) \<Ztypecolon> ?T ret \<^bold>t\<^bold>h\<^bold>r\<^bold>o\<^bold>w\<^bold>s ?E \<rbrace> \<^bold>@\<^bold>G\<^bold>O\<^bold>A\<^bold>L ?G\<close>
 ]:
   assumes F1: \<open>\<^bold>p\<^bold>r\<^bold>o\<^bold>c f1 \<lbrace> R  \<longmapsto> R1\<heavy_comma> SYNTHESIS \<^bold>v\<^bold>a\<^bold>l y \<Ztypecolon> \<bool> \<^bold>t\<^bold>h\<^bold>r\<^bold>o\<^bold>w\<^bold>s E1 \<rbrace>  \<^bold>@\<^bold>G\<^bold>O\<^bold>A\<^bold>L G\<close>
@@ -213,7 +212,7 @@ proc "\<phi>__synthesis_land"[
   argument \<open>R\<close>
   return   \<open>R2\<heavy_comma> SYNTHESIS \<^bold>v\<^bold>a\<^bold>l (x \<and> y) \<Ztypecolon> \<bool>\<close>
   throws   \<open>E1 + E2\<close>
-  \<medium_left_bracket> F1 \<rightarrow> y;; F2 $y \<and> \<medium_right_bracket>. .
+  \<medium_left_bracket> F1 F2 \<and> \<medium_right_bracket>. .
 
 paragraph \<open>Or\<close>
 
@@ -223,7 +222,7 @@ lemma (in std) op_or[\<phi>overload \<or>]:
   by (cases va; cases vb, simp, \<phi>reason)
 
 
-proc \<phi>__synthesis_lor[
+proc [
     \<phi>reason on \<open>\<^bold>p\<^bold>r\<^bold>o\<^bold>c ?F \<lbrace> ?R \<longmapsto> \<lambda>ret. ?R2\<heavy_comma> SYNTHESIS (?x \<or> ?y) \<Ztypecolon> ?T ret \<^bold>t\<^bold>h\<^bold>r\<^bold>o\<^bold>w\<^bold>s ?E \<rbrace> \<^bold>@\<^bold>G\<^bold>O\<^bold>A\<^bold>L ?G\<close>
 ]:
   assumes F1: \<open>\<^bold>p\<^bold>r\<^bold>o\<^bold>c f1 \<lbrace> R \<longmapsto> R1\<heavy_comma> SYNTHESIS \<^bold>v\<^bold>a\<^bold>l y \<Ztypecolon> \<bool> \<^bold>t\<^bold>h\<^bold>r\<^bold>o\<^bold>w\<^bold>s E1 \<rbrace>  \<^bold>@\<^bold>G\<^bold>O\<^bold>A\<^bold>L G\<close>
@@ -232,7 +231,7 @@ proc \<phi>__synthesis_lor[
   argument \<open>R\<close>
   return   \<open>R2\<heavy_comma> SYNTHESIS \<^bold>v\<^bold>a\<^bold>l (x \<or> y) \<Ztypecolon> \<bool>\<close>
   throws \<open>E1 + E2\<close>
-  \<medium_left_bracket> F1 \<rightarrow> y;; F2 $y \<or> \<medium_right_bracket>. .
+  \<medium_left_bracket> F1 F2 \<or> \<medium_right_bracket>. .
 
 
 subsubsection \<open>Constant Integer\<close>
@@ -286,7 +285,7 @@ lemma (in std) op_add[\<phi>overload +]:
   unfolding op_add_def Premise_def
   by (cases vx; cases vy; simp, \<phi>reason)
 
-proc \<phi>__synthesis_add[
+proc [
     \<phi>reason on \<open>\<^bold>p\<^bold>r\<^bold>o\<^bold>c ?F \<lbrace> ?R \<longmapsto> \<lambda>ret. ?R2\<heavy_comma> SYNTHESIS (?x + ?y) \<Ztypecolon> ?T ret \<^bold>t\<^bold>h\<^bold>r\<^bold>o\<^bold>w\<^bold>s ?E \<rbrace> \<^bold>@\<^bold>G\<^bold>O\<^bold>A\<^bold>L ?G\<close>
 ]:
   assumes F1: \<open>\<^bold>p\<^bold>r\<^bold>o\<^bold>c f1 \<lbrace> R \<longmapsto> R1\<heavy_comma> SYNTHESIS \<^bold>v\<^bold>a\<^bold>l x \<Ztypecolon> \<nat>[b]  \<^bold>t\<^bold>h\<^bold>r\<^bold>o\<^bold>w\<^bold>s E1 \<rbrace>  \<^bold>@\<^bold>G\<^bold>O\<^bold>A\<^bold>L G\<close>
@@ -296,7 +295,7 @@ proc \<phi>__synthesis_add[
   argument \<open>R\<close>
   return   \<open>R2\<heavy_comma> SYNTHESIS \<^bold>v\<^bold>a\<^bold>l (x + y) \<Ztypecolon> \<nat>[b]\<close>
   throws \<open>E1 + E2\<close>
-  \<medium_left_bracket> F1 \<rightarrow> x;; F2 \<rightarrow> y;; $x $y + \<medium_right_bracket>. .
+  \<medium_left_bracket> F1 F2 + \<medium_right_bracket>. .
 
 
 paragraph \<open>Subtraction\<close>
@@ -309,7 +308,7 @@ lemma (in std) op_sub[\<phi>overload -]:
   apply (simp add: \<phi>expns)
   by (metis Nat.add_diff_assoc2 add.commute less_imp_diff_less mod_add_self2 mod_less)
 
-proc \<phi>__synthesis_sub[
+proc [
     \<phi>reason on \<open>\<^bold>p\<^bold>r\<^bold>o\<^bold>c ?F \<lbrace> ?R \<longmapsto> \<lambda>ret. ?R2\<heavy_comma> SYNTHESIS (?x - ?y) \<Ztypecolon> ?T ret \<^bold>t\<^bold>h\<^bold>r\<^bold>o\<^bold>w\<^bold>s ?E \<rbrace> \<^bold>@\<^bold>G\<^bold>O\<^bold>A\<^bold>L ?G\<close>
 ]:
   assumes F1: \<open>\<^bold>p\<^bold>r\<^bold>o\<^bold>c f1 \<lbrace> R \<longmapsto> R1\<heavy_comma> SYNTHESIS \<^bold>v\<^bold>a\<^bold>l x \<Ztypecolon> \<nat>[b] \<^bold>t\<^bold>h\<^bold>r\<^bold>o\<^bold>w\<^bold>s E1 \<rbrace>  \<^bold>@\<^bold>G\<^bold>O\<^bold>A\<^bold>L G\<close>
@@ -319,7 +318,29 @@ proc \<phi>__synthesis_sub[
   argument \<open>R\<close>
   return   \<open>R2\<heavy_comma> SYNTHESIS \<^bold>v\<^bold>a\<^bold>l (x - y) \<Ztypecolon> \<nat>[b]\<close>
   throws \<open>E1 + E2\<close>
-  \<medium_left_bracket> F1 \<rightarrow> x;; F2 \<rightarrow> y;; $x $y - \<medium_right_bracket>. .
+  \<medium_left_bracket> F1 F2 - \<medium_right_bracket>. .
+
+
+paragraph \<open>Times\<close>
+
+lemma (in std) op_omul[\<phi>overload *]:
+  \<open> \<^bold>p\<^bold>r\<^bold>e\<^bold>m\<^bold>i\<^bold>s\<^bold>e x * y < 2^b
+\<Longrightarrow> \<^bold>p\<^bold>r\<^bold>o\<^bold>c op_umul b (\<phi>V_pair vy vx) \<lbrace> x \<Ztypecolon> Val vx \<nat>[b]\<heavy_comma> y \<Ztypecolon> Val vy \<nat>[b] \<longmapsto> \<^bold>v\<^bold>a\<^bold>l x * y \<Ztypecolon> \<nat>[b] \<rbrace>\<close>
+  unfolding op_umul_def Premise_def
+  by (cases vx; cases vy; simp, \<phi>reason)
+
+proc [
+    \<phi>reason on \<open>\<^bold>p\<^bold>r\<^bold>o\<^bold>c ?F \<lbrace> ?R \<longmapsto> \<lambda>ret. ?R2\<heavy_comma> SYNTHESIS (?x * ?y) \<Ztypecolon> ?T ret \<^bold>t\<^bold>h\<^bold>r\<^bold>o\<^bold>w\<^bold>s ?E \<rbrace> \<^bold>@\<^bold>G\<^bold>O\<^bold>A\<^bold>L ?G\<close>
+]:
+  assumes F1: \<open>\<^bold>p\<^bold>r\<^bold>o\<^bold>c f1 \<lbrace> R \<longmapsto> R1\<heavy_comma> SYNTHESIS \<^bold>v\<^bold>a\<^bold>l x \<Ztypecolon> \<nat>[b] \<^bold>t\<^bold>h\<^bold>r\<^bold>o\<^bold>w\<^bold>s E1 \<rbrace>  \<^bold>@\<^bold>G\<^bold>O\<^bold>A\<^bold>L G\<close>
+    and   F2: \<open>\<^bold>p\<^bold>r\<^bold>o\<^bold>c f2 \<lbrace> R1 \<longmapsto> R2\<heavy_comma> SYNTHESIS \<^bold>v\<^bold>a\<^bold>l y \<Ztypecolon> \<nat>[b] \<^bold>t\<^bold>h\<^bold>r\<^bold>o\<^bold>w\<^bold>s E2 \<rbrace>  \<^bold>@\<^bold>G\<^bold>O\<^bold>A\<^bold>L G\<close>
+  premises \<open>x*y < 2^b\<close>
+  goal G
+  argument \<open>R\<close>
+  return   \<open>R2\<heavy_comma> SYNTHESIS \<^bold>v\<^bold>a\<^bold>l (x * y) \<Ztypecolon> \<nat>[b]\<close>
+  throws \<open>E1 + E2\<close>
+  \<medium_left_bracket> F1 F2 * \<medium_right_bracket>. .
+
 
 
 paragraph \<open>Division\<close>
@@ -330,7 +351,7 @@ lemma (in std) op_udiv[\<phi>overload /]:
   apply (cases vx; cases vy; simp, \<phi>reason) apply (simp add: \<phi>expns)
   using div_le_dividend le_less_trans by blast
 
-proc \<phi>__synthesis_udiv[
+proc [
     \<phi>reason on \<open>\<^bold>p\<^bold>r\<^bold>o\<^bold>c ?F \<lbrace> ?R \<longmapsto> \<lambda>ret. ?R2\<heavy_comma> SYNTHESIS (?x div ?y) \<Ztypecolon> ?T ret \<^bold>t\<^bold>h\<^bold>r\<^bold>o\<^bold>w\<^bold>s ?E \<rbrace> \<^bold>@\<^bold>G\<^bold>O\<^bold>A\<^bold>L ?G\<close>
 ]:
   assumes F1: \<open>\<^bold>p\<^bold>r\<^bold>o\<^bold>c f1 \<lbrace> R \<longmapsto> R1\<heavy_comma> SYNTHESIS \<^bold>v\<^bold>a\<^bold>l x \<Ztypecolon> \<nat>[b] \<^bold>t\<^bold>h\<^bold>r\<^bold>o\<^bold>w\<^bold>s E1 \<rbrace>  \<^bold>@\<^bold>G\<^bold>O\<^bold>A\<^bold>L G\<close>
@@ -339,7 +360,7 @@ proc \<phi>__synthesis_udiv[
   argument \<open>R\<close>
   return   \<open>R2\<heavy_comma> SYNTHESIS \<^bold>v\<^bold>a\<^bold>l (x div y) \<Ztypecolon> \<nat>[b]\<close>
   throws \<open>E1 + E2\<close>
-  \<medium_left_bracket> F1 \<rightarrow> x;; F2 \<rightarrow> y;; $x $y / \<medium_right_bracket>. .
+  \<medium_left_bracket> F1 F2 / \<medium_right_bracket>. .
 
 
 paragraph \<open>Less Than\<close>
@@ -349,22 +370,18 @@ lemma (in std) op_lt[\<phi>overload <]:
   unfolding op_lt_def
   by (cases rawx; cases rawy; simp, \<phi>reason)
 
-
-proc \<phi>__synthesis_lt[
+proc [
     \<phi>reason on \<open>\<^bold>p\<^bold>r\<^bold>o\<^bold>c ?F \<lbrace> ?R \<longmapsto> \<lambda>ret. ?R2\<heavy_comma> SYNTHESIS (?x < ?y) \<Ztypecolon> ?T ret \<^bold>t\<^bold>h\<^bold>r\<^bold>o\<^bold>w\<^bold>s ?E \<rbrace> \<^bold>@\<^bold>G\<^bold>O\<^bold>A\<^bold>L ?G\<close>
 ]:
-  assumes F1: \<open>\<^bold>p\<^bold>r\<^bold>o\<^bold>c f1 \<lbrace> R \<longmapsto> R1\<heavy_comma> \<^bold>v\<^bold>a\<^bold>l xxx \<Ztypecolon> \<nat>[b]\<heavy_comma> \<^bold>v\<^bold>a\<^bold>l yyy \<Ztypecolon> \<bool>\<heavy_comma> SYNTHESIS \<^bold>v\<^bold>a\<^bold>l x \<Ztypecolon> \<nat>[b] \<^bold>t\<^bold>h\<^bold>r\<^bold>o\<^bold>w\<^bold>s E1 \<rbrace>  \<^bold>@\<^bold>G\<^bold>O\<^bold>A\<^bold>L G\<close>
+  assumes F1: \<open>\<^bold>p\<^bold>r\<^bold>o\<^bold>c f1 \<lbrace> R  \<longmapsto> R1\<heavy_comma> SYNTHESIS \<^bold>v\<^bold>a\<^bold>l x \<Ztypecolon> \<nat>[b] \<^bold>t\<^bold>h\<^bold>r\<^bold>o\<^bold>w\<^bold>s E1 \<rbrace>  \<^bold>@\<^bold>G\<^bold>O\<^bold>A\<^bold>L G\<close>
     and   F2: \<open>\<^bold>p\<^bold>r\<^bold>o\<^bold>c f2 \<lbrace> R1 \<longmapsto> R2\<heavy_comma> SYNTHESIS \<^bold>v\<^bold>a\<^bold>l y \<Ztypecolon> \<nat>[b] \<^bold>t\<^bold>h\<^bold>r\<^bold>o\<^bold>w\<^bold>s E2 \<rbrace>  \<^bold>@\<^bold>G\<^bold>O\<^bold>A\<^bold>L G\<close>
   goal G
   argument \<open>R\<close>
   return   \<open>R2\<heavy_comma> SYNTHESIS \<^bold>v\<^bold>a\<^bold>l (x < y) \<Ztypecolon> \<bool>\<close>
   throws \<open>E1 + E2\<close>
-  \<medium_left_bracket> \<open>0 \<Ztypecolon> \<nat>[b]\<close> \<rightarrow>  x  ;;
- F1;; \<rightarrow> x'', x',  x
-  ;; F2 \<rightarrow> y ;; $x $y < \<medium_right_bracket>
-  .. .
+  \<medium_left_bracket> F1 F2 < \<medium_right_bracket>. .
 
-proc \<phi>__synthesis_gt[
+proc [
     \<phi>reason on \<open>\<^bold>p\<^bold>r\<^bold>o\<^bold>c ?F \<lbrace> ?R \<longmapsto> \<lambda>ret. ?R2\<heavy_comma> SYNTHESIS (?x > ?y) \<Ztypecolon> ?T ret \<^bold>t\<^bold>h\<^bold>r\<^bold>o\<^bold>w\<^bold>s ?E \<rbrace> \<^bold>@\<^bold>G\<^bold>O\<^bold>A\<^bold>L ?G\<close>
 ]:
   assumes F1: \<open>\<^bold>p\<^bold>r\<^bold>o\<^bold>c f1 \<lbrace> R \<longmapsto> R1\<heavy_comma> SYNTHESIS \<^bold>v\<^bold>a\<^bold>l x \<Ztypecolon> \<nat>[b] \<^bold>t\<^bold>h\<^bold>r\<^bold>o\<^bold>w\<^bold>s E1 \<rbrace>  \<^bold>@\<^bold>G\<^bold>O\<^bold>A\<^bold>L G\<close>
@@ -373,7 +390,7 @@ proc \<phi>__synthesis_gt[
   argument \<open>R\<close>
   return   \<open>R2\<heavy_comma> SYNTHESIS \<^bold>v\<^bold>a\<^bold>l (x > y) \<Ztypecolon> \<bool>\<close>
   throws \<open>E1 + E2\<close>
-  \<medium_left_bracket> F1 \<rightarrow> y;; F2 $y < \<medium_right_bracket>. .
+  \<medium_left_bracket> F1 F2 \<open>\<v>\<a>\<l>1\<close> \<open>\<v>\<a>\<l>0\<close> < \<medium_right_bracket>. .
 
 paragraph \<open>Less Equal\<close>
 
@@ -382,7 +399,7 @@ lemma (in std) op_le[\<phi>overload \<le>]:
   unfolding op_le_def
   by (cases rawx; cases rawy; simp, \<phi>reason)
 
-proc \<phi>__synthesis_le[
+proc [
     \<phi>reason on \<open>\<^bold>p\<^bold>r\<^bold>o\<^bold>c ?F \<lbrace> ?R \<longmapsto> \<lambda>ret. ?R2\<heavy_comma> SYNTHESIS (?x \<le> ?y) \<Ztypecolon> ?T ret \<^bold>t\<^bold>h\<^bold>r\<^bold>o\<^bold>w\<^bold>s ?E \<rbrace> \<^bold>@\<^bold>G\<^bold>O\<^bold>A\<^bold>L ?G\<close>
 ]:
   assumes F1: \<open>\<^bold>p\<^bold>r\<^bold>o\<^bold>c f1 \<lbrace> R \<longmapsto> R1\<heavy_comma> SYNTHESIS \<^bold>v\<^bold>a\<^bold>l x \<Ztypecolon> \<nat>[b]  \<^bold>t\<^bold>h\<^bold>r\<^bold>o\<^bold>w\<^bold>s E1 \<rbrace>  \<^bold>@\<^bold>G\<^bold>O\<^bold>A\<^bold>L G\<close>
@@ -391,9 +408,9 @@ proc \<phi>__synthesis_le[
   argument \<open>R\<close>
   return   \<open>R2\<heavy_comma> SYNTHESIS \<^bold>v\<^bold>a\<^bold>l (x \<le> y) \<Ztypecolon> \<bool>\<close>
   throws \<open>E1 + E2\<close>
-  \<medium_left_bracket> F1 \<rightarrow> x;; F2 \<rightarrow> y;; $x $y \<le> \<medium_right_bracket>. .
+  \<medium_left_bracket> F1 F2 \<le> \<medium_right_bracket>. .
 
-proc \<phi>__synthesis_ge[
+proc [
     \<phi>reason on \<open>\<^bold>p\<^bold>r\<^bold>o\<^bold>c ?F \<lbrace> ?R \<longmapsto> \<lambda>ret. ?R2\<heavy_comma> SYNTHESIS (?x \<ge> ?y) \<Ztypecolon> ?T ret \<^bold>t\<^bold>h\<^bold>r\<^bold>o\<^bold>w\<^bold>s ?E \<rbrace> \<^bold>@\<^bold>G\<^bold>O\<^bold>A\<^bold>L ?G\<close>
 ]:
   assumes F1: \<open>\<^bold>p\<^bold>r\<^bold>o\<^bold>c f1 \<lbrace> R \<longmapsto> R1\<heavy_comma> SYNTHESIS \<^bold>v\<^bold>a\<^bold>l x \<Ztypecolon> \<nat>[b] \<^bold>t\<^bold>h\<^bold>r\<^bold>o\<^bold>w\<^bold>s E1 \<rbrace>  \<^bold>@\<^bold>G\<^bold>O\<^bold>A\<^bold>L G\<close>
@@ -402,7 +419,7 @@ proc \<phi>__synthesis_ge[
   argument \<open>R\<close>
   return   \<open>R2\<heavy_comma> SYNTHESIS \<^bold>v\<^bold>a\<^bold>l (x \<ge> y) \<Ztypecolon> \<bool>\<close>
   throws \<open>E1 + E2\<close>
-  \<medium_left_bracket> F1 \<rightarrow> x;; F2 $x \<le> \<medium_right_bracket>. .
+  \<medium_left_bracket> F1 F2 \<open>\<v>\<a>\<l>1\<close> \<open>\<v>\<a>\<l>0\<close> \<le> \<medium_right_bracket>. .
 
 
 subsubsection \<open>General Arithmetic\<close>
@@ -562,9 +579,9 @@ proc while:
 proc AA:
   argument \<open>\<^bold>v\<^bold>a\<^bold>l 1 \<Ztypecolon> \<nat>[32]\<heavy_comma> \<^bold>v\<^bold>a\<^bold>l 2 \<Ztypecolon> \<nat>[32]\<heavy_comma> \<^bold>v\<^bold>a\<^bold>l 3 \<Ztypecolon> \<nat>[32]\<close>
   return \<open>\<^bold>v\<^bold>a\<^bold>l 6 \<Ztypecolon> \<nat>[32]\<heavy_comma> \<^bold>v\<^bold>a\<^bold>l 4 \<Ztypecolon> \<nat>[32]\<heavy_comma> \<^bold>v\<^bold>a\<^bold>l 2 \<Ztypecolon> \<nat>[32]\<close>
-  \<medium_left_bracket> + + 4 2
-  \<medium_right_bracket>. .
+  \<medium_left_bracket>  + + 4 2 1 - 1 + 30000 * 30000 /  \<medium_right_bracket>. .
 
+thm op_const_int_\<phi>app
 thm AA_\<phi>compilation
 
 proc XX:
@@ -579,6 +596,7 @@ proc XX:
        to make that value automatically *)
   \<medium_right_bracket>. .
 
+thm XX_\<phi>compilation
 
 proc
   premises \<open>x < 10\<close>
